@prefix bf: <http://id.loc.gov/ontologies/bibframe/> .
@prefix bflc: <http://id.loc.gov/ontologies/bflc/> .
@prefix cc: <http://creativecommons.org/ns#> .
@prefix dcterms: <http://purl.org/dc/terms/> .
@prefix foaf: <http://xmlns.com/foaf/0.1/> .
@prefix owl: <http://www.w3.org/2002/07/owl#> .
@prefix rdf: <http://www.w3.org/1999/02/22-rdf-syntax-ns#> .
@prefix rdfs: <http://www.w3.org/2000/01/rdf-schema#> .
@prefix skos: <http://www.w3.org/2004/02/skos/core#> .
@prefix xs: <http://www.w3.org/2001/XMLSchema#> .

<http://id.loc.gov/ontologies/bibframe/>
  a owl:Ontology ;
  rdfs:label "BIBFRAME vocabulary" ;
  cc:license <https://creativecommons.org/publicdomain/zero/1.0/> ;
  dcterms:creator [
    rdfs:resource "http://id.loc.gov/vocabulary/organizations/dlc" ;
  ] ;
  dcterms:description '''The Bibframe vocabulary consists of RDF classes and properties used for the description of 
            items cataloged principally by libraries, but may also be used to describe items cataloged by museums and archives. 
            Classes include the three core classes - Work, Instance, and Item - in addition to many more 
            classes to support description. Properties describe characteristics of the resource being 
            described as well as relationships among resources. For example: one Work
            might be a "translation of" another Work; an Instance may be an 
            "instance of" a particular Bibframe Work.  Other properties describe attributes of Works and Instances.  For
            example: the Bibframe property "subject" expresses an important attribute of a Work 
            (what the Work is about), and the property "extent" (e.g. number of pages) expresses an
            attribute of an Instance.'''@en ;
  dcterms:issued "2025-01-24T12:00:00.000-05:00"^^xs:dateTime ;
  dcterms:modified "2025-02-10T09:52:36.66620558-05:00"^^xs:dateTime ;
  dcterms:publisher [
    rdfs:resource "http://id.loc.gov/vocabulary/organizations/dlcmrc" ;
  ] ;
  dcterms:rights <https://creativecommons.org/publicdomain/zero/1.0/> ;
  owl:priorVersion <http://id.loc.gov/ontologies/bibframe-2-4-0/> ;
  owl:versionIRI <http://id.loc.gov/ontologies/bibframe-2-5-0/> ;
  owl:versionInfo "2.5.0" ;
  .

bf:AbbreviatedTitle
  a owl:Class ;
  rdfs:subClassOf bf:VariantTitle ;
  rdfs:label "Abbreviated title" ;
  dcterms:modified "2016-04-21 (New)" ;
  skos:definition "Title as abbreviated for citation, indexing, and/or identification" ;
  .

bf:AccessPolicy
  a owl:Class ;
  rdfs:subClassOf bf:UsageAndAccessPolicy ;
  rdfs:label "Access policy" ;
  dcterms:modified "2016-04-21 (New)" ;
  skos:definition "Access restrictions and allowances regarding access to a resource, e.g., lending policy, access restrictions, embargos" ;
  .

bf:AccessionNumber
  a owl:Class ;
  rdfs:subClassOf bf:Identifier ;
  rdfs:label "Accession number" ;
  dcterms:modified "2021-06-09 (New [GH11])" ;
  skos:definition "Accession Number" ;
  .

bf:AcquisitionSource
  a owl:Class ;
  rdfs:label "Acquisition source" ;
  dcterms:modified "2017-02-06 (New)" ;
  skos:definition "Information about an organization, person, etc., from which a resource may be obtained" ;
  .

bf:AdminMetadata
  a owl:Class ;
  rdfs:label "Administrative metadata" ;
  dcterms:modified "2016-04-21 (New)" ;
  skos:definition "Metadata about the metadata, especially provenance information" ;
  .

bf:Agent
  a owl:Class ;
  rdfs:subClassOf foaf:Agent ;
  rdfs:label "Agent" ;
  dcterms:modified
    "2016-04-21 (New)" ,
    "2016-05-13 (New subclass)"
    ;
  skos:definition "Entity having a role in a resource, such as a person or organization" ;
  .

bf:Ansi
  a owl:Class ;
  rdfs:subClassOf bf:Identifier ;
  rdfs:label "ANSI number" ;
  dcterms:modified "2016-04-21 (New)" ;
  skos:definition "American National Standards Institute identifier" ;
  .

bf:AppliedMaterial
  a owl:Class ;
  rdfs:subClassOf bf:Material ;
  rdfs:label "Applied material" ;
  dcterms:modified
    "2016-04-21 (New)" ,
    "2021-06-09 (Changed subclass to Material [GH28])"
    ;
  skos:definition "Physical or chemical substance applied to a base material of a resource" ;
  .

bf:Archival
  a owl:Class ;
  rdfs:subClassOf bf:Instance ;
  rdfs:label "Archival controlled" ;
  dcterms:modified "2016-04-21 (New)" ;
  skos:definition "Resources organically created, accumulated, and/or used by a person, family, or organization in the course of conduct of affairs and preserved because of their continuing value" ;
  .

bf:Arrangement
  a owl:Class ;
  rdfs:subClassOf bf:Work ;
  rdfs:label "Arrangement" ;
  dcterms:modified
    "2016-04-21 (New)" ,
    "2021-06-09 (Redefined [GH77])"
    ;
  skos:definition "Resource that represents an arrangement of another resource" ;
  .

bf:AspectRatio
  a owl:Class ;
  rdfs:label "Aspect ratio" ;
  dcterms:modified "2016-04-21 (New)" ;
  skos:definition "Proportional relationship between an image's width and its height" ;
  .

bf:Audio
  a owl:Class ;
  rdfs:subClassOf bf:Work ;
  rdfs:label "Audio" ;
  dcterms:modified "2016-04-21 (New)" ;
  skos:definition "Resources expressed in an audible form, including music or other sounds" ;
  .

bf:AudioIssueNumber
  a owl:Class ;
  rdfs:subClassOf bf:Identifier ;
  rdfs:label "Audio issue number" ;
  dcterms:modified
    "2016-04-21 (New)" ,
    "2017-02-03 (Revised property name and definition)"
    ;
  skos:definition "Number assigned by publishers of sound recordings to identify the issue designation, or serial identification, of the resource" ;
  .

bf:AudioTake
  a owl:Class ;
  rdfs:subClassOf bf:Identifier ;
  rdfs:label "Audio recording take" ;
  dcterms:modified "2017-02-03 (New)" ;
  skos:definition "Identifier assigned to the smallest identifiable unit of a recording session, e.g., a specific recording of an individual song" ;
  .

bf:Barcode
  a owl:Class ;
  rdfs:subClassOf bf:Identifier ;
  rdfs:label "Barcode" ;
  dcterms:modified
    "2016-04-21 (New)" ,
    "2017-02-03 (Moved to Identifier class group from Item group)"
    ;
  skos:definition "Optical machine-readable representation of data relating to the item to which it is attached" ;
  .

bf:BaseMaterial
  a owl:Class ;
  rdfs:subClassOf bf:Material ;
  rdfs:label "Base material" ;
  dcterms:modified
    "2016-04-21 (New)" ,
    "2021-06-09 (Changed subclass to Material [GH28])"
    ;
  skos:definition "Underlying physical material of a resource" ;
  .

bf:Binding
  a owl:Class ;
  rdfs:label "Binding method" ;
  dcterms:modified "2022-10-03 (New [GH91])" ;
  skos:definition "Information about methods used to bind a published or unpublished resource, or other binding information" ;
  .

bf:BookFormat
  a owl:Class ;
  rdfs:label "Book format" ;
  dcterms:modified "2016-04-21 (New)" ;
  skos:definition "Result of folding a printed sheet to form a gathering of leaves" ;
  .

bf:BroadcastStandard
  a owl:Class ;
  rdfs:subClassOf bf:VideoCharacteristic ;
  rdfs:label "Broadcast standard" ;
  dcterms:modified "2016-04-21 (New)" ;
  skos:definition "System used to format a video resource for television broadcast, e.g., HDTV, PAL" ;
  .

bf:Capture
  a owl:Class ;
  rdfs:label "Capture of content" ;
  dcterms:modified "2016-04-21 (New)" ;
  skos:definition "Information about place and date associated with the capture (i.e., recording, filming, etc.) of the content of a resource" ;
  .

bf:CaptureStorage
  a owl:Class ;
  rdfs:subClassOf bf:SoundCharacteristic ;
  rdfs:label "Capture and Storage Technique" ;
  dcterms:modified "2023-11-30 (New [GH104])" ;
  skos:definition "Specifies the sound capture and storage technique used on a sound recording resource" ;
  .

bf:Carrier
  a owl:Class ;
  rdfs:label "Carrier type" ;
  dcterms:modified "2016-04-21 (New)" ;
  skos:definition "Categorization reflecting the format of the storage medium and housing of a carrier" ;
  .

bf:Cartographic
  a owl:Class ;
  rdfs:label "Cartographic information" ;
  dcterms:modified "2016-04-21 (New)" ;
  skos:definition "Content that represents the whole or part of the earth, any celestial body, or imaginary place at any scale" ;
  .

bf:CartographicDataType
  a owl:Class ;
  rdfs:subClassOf bf:DigitalCharacteristic ;
  rdfs:label "Digital cartographic data type" ;
  dcterms:modified "2016-04-21 (New)" ;
  skos:definition "Data type for encoding of geospatial information in a cartographic resource, e.g., raster, vector, point" ;
  .

bf:CartographicObjectType
  a owl:Class ;
  rdfs:subClassOf bf:DigitalCharacteristic ;
  rdfs:label "Digital cartographic object type" ;
  dcterms:modified "2016-04-21 (New)" ;
  skos:definition "Object type for encoding of geospatial information in a cartographic resource, e.g., point, line, polygon" ;
  .

bf:Cartography
  a owl:Class ;
  rdfs:subClassOf bf:Work ;
  rdfs:label "Cartography" ;
  dcterms:modified "2016-04-25 (fixed typo in definition)" ;
  skos:definition "Resource that shows spatial information, including maps, atlases, globes, digital, and other cartographic resources" ;
  .

bf:Chronology
  a owl:Class ;
  rdfs:subClassOf bf:EnumerationAndChronology ;
  rdfs:label "Chronology" ;
  dcterms:modified "2016-04-21 (New)" ;
  skos:definition "Dates associated with issues or items held" ;
  .

bf:Classification
  a owl:Class ;
  rdfs:label "Classification entity" ;
  dcterms:modified
    "2016-04-21 (New)" ,
    "2021-06-09 (Added editorial note [GH55])"
    ;
  skos:definition "System of coding and organizing materials according to their subject" ;
  skos:editorialNote "Any entry from the Classification Schemes vocabulary at ID may be used; all have been defined as a bf:Classification" ;
  .

bf:ClassificationDdc
  a owl:Class ;
  rdfs:subClassOf bf:Classification ;
  rdfs:label "DDC Classification" ;
  dcterms:modified "2016-04-21 (New)" ;
  skos:definition "Dewey Decimal Classification number used for subject access" ;
  .

bf:ClassificationLcc
  a owl:Class ;
  rdfs:subClassOf bf:Classification ;
  rdfs:label "LCC Classification" ;
  dcterms:modified "2016-04-21 (New)" ;
  skos:definition "Library of Congress Classification number used for subject access" ;
  .

bf:ClassificationNal
  a owl:Class ;
  rdfs:subClassOf bf:Classification ;
  rdfs:label "NAL classification" ;
  dcterms:modified "2024-07-10 (New [GH119])" ;
  skos:definition "National Library of Agriculter number used for subject access" ;
  .

bf:ClassificationNlm
  a owl:Class ;
  rdfs:subClassOf bf:Classification ;
  rdfs:label "NLM classification" ;
  dcterms:modified "2016-04-21 (New)" ;
  skos:definition "National Library of Medicine Classification number used for subject access" ;
  .

bf:ClassificationUdc
  a owl:Class ;
  rdfs:subClassOf bf:Classification ;
  rdfs:label "UDC Classification" ;
  dcterms:modified "2016-04-21 (New)" ;
  skos:definition "Universal Decimal Classification number used for subject access" ;
  .

bf:Coden
  a owl:Class ;
  rdfs:subClassOf bf:Identifier ;
  rdfs:label "CODEN" ;
  dcterms:modified "2016-04-21 (New)" ;
  skos:definition "Identifier for scientific and technical periodical titles assigned by the International CODEN Section of Chemical Abstracts Service" ;
  .

bf:Collection
  a owl:Class ;
  rdfs:subClassOf bf:Work ;
  rdfs:label "Collection" ;
  dcterms:modified
    "2016-04-21 (New)" ,
    "2022-10-03 (changed subClassOf [GH92])"
    ;
  skos:definition "Aggregation of resources, generally gathered together artificially" ;
  .

bf:CollectionArrangement
  a owl:Class ;
  rdfs:label "Organization of materials information" ;
  dcterms:modified "2021-06-09 (New [GH77])" ;
  skos:definition "Information about the organization and arrangement of a collection of items" ;
  .

bf:CollectiveTitle
  a owl:Class ;
  rdfs:subClassOf bf:VariantTitle ;
  rdfs:label "Collective title" ;
  dcterms:modified "2016-04-21 (New)" ;
  skos:definition "Title for a compilation of resources" ;
  .

bf:ColorContent
  a owl:Class ;
  rdfs:label "Color content" ;
  dcterms:modified "2016-04-21 (New)" ;
  skos:definition "Color characteristics of a resource, e.g., black and white, multicolored, etc." ;
  .

bf:Content
  a owl:Class ;
  rdfs:label "Content type" ;
  dcterms:modified "2016-04-21 (New)" ;
  skos:definition "Categorization reflecting the fundamental form of communication in which the content is expressed and the human sense through which it is intended to be perceived" ;
  .

bf:ContentAccessibility
  a owl:Class ;
  rdfs:label "Content accessibility information" ;
  dcterms:modified "2017-02-07 (New)" ;
  skos:definition "Information that assists those with a sensory impairment for greater understanding of content, e.g., captions" ;
  .

bf:Contribution
  a owl:Class ;
  rdfs:label "Contribution" ;
  dcterms:modified "2016-04-21 (New)" ;
  skos:definition "Agent and role with respect to the resource being described" ;
  .

bf:CopyrightNumber
  a owl:Class ;
  rdfs:subClassOf bf:Identifier ;
  rdfs:label "Copyright-legal deposit number" ;
  dcterms:modified "2016-04-21 (New)" ;
  skos:definition "Identifier assigned to a copyright registration or legal deposit" ;
  .

bf:CopyrightRegistration
  a owl:Class ;
  rdfs:label "Copyright registration" ;
  dcterms:modified
    "2016-04-21 (New)" ,
    "2016-05-04 (Class name corrected)"
    ;
  skos:definition "Copyright or Legal Deposit registration information" ;
  .

bf:CoverArt
  a owl:Class ;
  rdfs:label "Cover art" ;
  dcterms:modified "2016-04-21 (New)" ;
  skos:definition "Cover illustration of a resource" ;
  .

bf:Dataset
  a owl:Class ;
  rdfs:subClassOf bf:Work ;
  rdfs:label "Dataset" ;
  dcterms:modified "2016-04-21 (New)" ;
  skos:definition "Data encoded in a defined structure, including numeric data, environmental data, etc., used by applications software" ;
  .

bf:DescriptionAuthentication
  a owl:Class ;
  rdfs:label "Metadata authentication" ;
  dcterms:modified
    "2016-04-21 (New)" ,
    "2016-04-29 (fixed class name)" ,
    "2022-10-03 (removed subClassOf [GH90])"
    ;
  skos:definition "Indication of specific types of reviews that have been carried out on the description information" ;
  .

bf:DescriptionConventions
  a owl:Class ;
  rdfs:label "Description conventions" ;
  dcterms:modified
    "2016-04-21 (New)" ,
    "2016-04-24 (fixed class name)" ,
    "2022-10-03 (removed subClassOf [GH90])"
    ;
  skos:definition "Rules used for the descriptive content of the resource description" ;
  .

bf:DescriptionLevel
  a owl:Class ;
  rdfs:label "Description level" ;
  dcterms:modified "2022-10-03 (New [GH43])" ;
  skos:definition "Designation of the descriptive content of the metadata" ;
  .

bf:DigitalCharacteristic
  a owl:Class ;
  rdfs:label "Digital characteristic" ;
  dcterms:modified "2016-04-21 (New)" ;
  skos:definition "Technical specification relating to the digital encoding of text, image, audio, video, and other types of data in a resource" ;
  .

bf:Dissertation
  a owl:Class ;
  rdfs:label "Dissertation information" ;
  dcterms:modified "2016-04-21 (New)" ;
  skos:definition "Information about a work presented as part of the formal requirements for an academic degree" ;
  .

bf:DissertationIdentifier
  a owl:Class ;
  rdfs:subClassOf bf:Identifier ;
  rdfs:label "Dissertation Identifier" ;
  dcterms:modified "2016-04-21 (New)" ;
  skos:definition "Identifier assigned to a thesis or dissertation for identification purposes" ;
  .

bf:Distribution
  a owl:Class ;
  rdfs:subClassOf bf:ProvisionActivity ;
  rdfs:label "Distributor" ;
  dcterms:modified "2016-04-21 (New)" ;
  skos:definition "Information relating to distribution of a resource" ;
  .

bf:Doi
  a owl:Class ;
  rdfs:subClassOf bf:Identifier ;
  rdfs:label "DOI" ;
  dcterms:modified "2016-04-21 (New)" ;
  skos:definition "Digital Object Identifier" ;
  .

bf:Ean
  a owl:Class ;
  rdfs:subClassOf bf:Identifier ;
  rdfs:label "EAN" ;
  dcterms:modified "2016-04-21 (New)" ;
  skos:definition "International Article Identifier" ;
  .

bf:Eidr
  a owl:Class ;
  rdfs:subClassOf bf:Identifier ;
  rdfs:label "EIDR" ;
  dcterms:modified "2021-06-09 (New [GH78])" ;
  skos:definition "Entertainment Identifier Registry" ;
  .

bf:Electronic
  a owl:Class ;
  rdfs:subClassOf bf:Instance ;
  rdfs:label "Electronic" ;
  dcterms:modified "2016-04-21 (New)" ;
  skos:definition "Resource that is intended for manipulation by a computer, accessed either directly or remotely" ;
  .

bf:Emulsion
  a owl:Class ;
  rdfs:label "Emulsion" ;
  dcterms:modified "2016-04-21 (New)" ;
  skos:definition "Suspension of light-sensitive chemicals used as a coating on a microfilm or microfiche, e.g., silver halide" ;
  .

bf:EncodedBitrate
  a owl:Class ;
  rdfs:subClassOf bf:DigitalCharacteristic ;
  rdfs:label "Encoded bitrate" ;
  dcterms:modified "2016-04-21 (New)" ;
  skos:definition "Speed at which streaming audio, video, etc., is designed to play, e.g., 32 kbps" ;
  .

bf:EncodingFormat
  a owl:Class ;
  rdfs:subClassOf bf:DigitalCharacteristic ;
  rdfs:label "Encoding format" ;
  dcterms:modified "2016-04-21 (New)" ;
  skos:definition "Schema, standard, etc., used to encode the digital content of a resource, e.g., MP3, XML, JPEG" ;
  .

bf:Ensemble
  a owl:Class ;
  rdfs:label "Ensemble" ;
  dcterms:modified "2021-06-09 (New [GH56])" ;
  skos:definition "Ensemble" ;
  .

bf:Enumeration
  a owl:Class ;
  rdfs:subClassOf bf:EnumerationAndChronology ;
  rdfs:label "Enumeration" ;
  dcterms:modified "2016-04-21 (New)" ;
  skos:definition "Numbering or other enumeration associated with issues or items held" ;
  .

bf:EnumerationAndChronology
  a owl:Class ;
  rdfs:label "Enumeration and chronology" ;
  dcterms:modified "2016-04-21 (New)" ;
  skos:definition "Numbering or other enumeration and dates associated with issues or items held" ;
  .

bf:Event
  a owl:Class ;
  rdfs:label "Event entity" ;
  dcterms:modified
    "2016-04-21 (New)" ,
    "2021-06-09 (Broaden definition [GH12])"
    ;
  skos:definition "Something that happens at a certain time and location, such as a performance, speech, or athletic event" ;
  .

bf:Extent
  a owl:Class ;
  rdfs:label "Extent" ;
  dcterms:modified "2016-04-21 (New)" ;
  skos:definition "Number and type of units and/or subunits making up a resource" ;
  .

bf:Family
  a owl:Class ;
  rdfs:subClassOf bf:Agent ;
  rdfs:label "Family" ;
  dcterms:modified "2016-04-21 (New)" ;
  skos:definition "Two or more persons related by birth, marriage, adoption, civil union, or similar legal status, or who otherwise present themselves as a family" ;
  .

bf:FileSize
  a owl:Class ;
  rdfs:subClassOf bf:DigitalCharacteristic ;
  rdfs:label "File size" ;
  dcterms:modified "2016-04-21 (New)" ;
  skos:definition "Number of bytes in a digital file, e.g., 162 KB" ;
  .

bf:FileType
  a owl:Class ;
  rdfs:subClassOf bf:DigitalCharacteristic ;
  rdfs:label "File type" ;
  dcterms:modified "2016-04-21 (New)" ;
  skos:definition "General type of data content encoded in a computer file, e.g., text file, audio file" ;
  .

bf:Fingerprint
  a owl:Class ;
  rdfs:subClassOf bf:Identifier ;
  rdfs:label "Fingerprint identifier" ;
  dcterms:modified "2016-04-21 (New)" ;
  skos:definition "Identifier that is used to assist in the identification of antiquarian books by recording information comprising groups of characters taken from specified positions on specified pages of the book" ;
  .

bf:FontSize
  a owl:Class ;
  rdfs:label "Font size" ;
  dcterms:modified "2016-04-21 (New)" ;
  skos:definition "Size of the type used to represent the characters and symbols in a resource" ;
  .

bf:Frequency
  a owl:Class ;
  rdfs:label "Frequency" ;
  dcterms:modified "2016-04-21 (New)" ;
  skos:definition "Information about intervals at which the parts of a serially produced resource or the updates to an integrating resource are issued" ;
  .

bf:Generation
  a owl:Class ;
  rdfs:label "Generation" ;
  dcterms:modified "2016-04-21 (New)" ;
  skos:definition "Relationship between an original carrier and the carrier of a reproduction made from the original" ;
  .

bf:GenerationProcess
  a owl:Class ;
  rdfs:label "Generation process" ;
  dcterms:modified
    "2016-04-21 (New)" ,
    "2016-04-24 (fixed class name)" ,
    "2022-10-03 (removed subClassOf [GH90])"
    ;
  skos:definition "Indication of the program or process used to generate the description by application of a particular transformation" ;
  .

bf:GenreForm
  a owl:Class ;
  rdfs:label "Genre/form" ;
  dcterms:modified
    "2016-04-21 (New)" ,
    "2021-06-09 (Broaden definition [GH17])"
    ;
  skos:definition "Form category or genre to which a resource belongs" ;
  .

bf:GeographicCoverage
  a owl:Class ;
  rdfs:label "Geographic coverage" ;
  dcterms:modified "2017-02-06 (New)" ;
  skos:definition "Geographic coverage of the content of the resource" ;
  .

bf:GrooveCharacteristic
  a owl:Class ;
  rdfs:subClassOf bf:SoundCharacteristic ;
  rdfs:label "Groove characteristic" ;
  dcterms:modified
    "2016-04-21 (New)" ,
    "2016-04-26 (fixed typo in definition)" ,
    "2017-02-03 (Fixed name of property)"
    ;
  skos:definition "Groove width of an analog disc or the groove pitch of an analog cylinder, e.g., coarse groove, microgroove" ;
  .

bf:Gtin14Number
  a owl:Class ;
  rdfs:subClassOf bf:Identifier ;
  rdfs:label "Global Trade Item Number 14" ;
  dcterms:modified "2017-02-03 (New)" ;
  skos:definition "14-digit number assigned to identify trade items as various packaging levels that encompasses EAN/UCC-128 and ITF-14" ;
  .

bf:Hdl
  a owl:Class ;
  rdfs:subClassOf bf:Identifier ;
  rdfs:label "Handle" ;
  dcterms:modified "2016-04-21 (New)" ;
  skos:definition "Unique and persistent identifier for digital objects developed by the Corporation for National Research Initiatives" ;
  .

bf:Hub
  a owl:Class ;
  rdfs:label "Hub" ;
  dcterms:modified
    "2021-06-09 (New [GH75])" ,
    "2023-11-30 (moved to Basic Model Class [GH108])"
    ;
  skos:definition "An abstract resource that functions as a bridge between two Works" ;
  .

bf:Identifier
  a owl:Class ;
  rdfs:label "Identifier" ;
  dcterms:modified
    "2016-04-21 (New)" ,
    "2021-06-09 (Added editorial note [GH44])"
    ;
  skos:definition "Token or name that is associated with a resource, such as a URI or an ISBN" ;
  skos:editorialNote "Any entry from the Standard Identifiers vocabulary at ID may be used; all have been defined as a bf:Identifier" ;
  .

bf:Illustration
  a owl:Class ;
  rdfs:label "Illustrative content" ;
  dcterms:modified "2016-04-21 (New)" ;
  skos:definition "Information about content intended to illustrate a resource" ;
  .

bf:ImmediateAcquisition
  a owl:Class ;
  rdfs:label "Immediate acquisition" ;
  dcterms:modified "2017-02-06 (New)" ;
  skos:definition "Information about the circumstances, e.g., source, date, method, under which the resource was directly acquired" ;
  .

bf:Instance
  a owl:Class ;
  rdfs:label "Instance" ;
  dcterms:modified "2016-04-21 (New)" ;
  skos:definition "Resource reflecting an individual, material embodiment of a Work" ;
  .

bf:Integrating
  a owl:Class ;
  rdfs:subClassOf bf:Work ;
  rdfs:label "Integrating resource" ;
  dcterms:modified "2022-10-03 (New [GH91])" ;
  skos:definition "Resource that is added to or changed by updates that do not remain discrete but are integrated into the whole" ;
  .

bf:IntendedAudience
  a owl:Class ;
  rdfs:label "Intended audience information" ;
  dcterms:modified "2016-04-21 (New)" ;
  skos:definition "Information that identifies the specific intended or target audience or intellectual level for which the content described is considered appropriate; also used to record interest and motivation levels and special learner characteristics" ;
  .

bf:Isan
  a owl:Class ;
  rdfs:subClassOf bf:Identifier ;
  rdfs:label "ISAN" ;
  dcterms:modified "2016-04-21 (New)" ;
  skos:definition "International Standard Audiovisual Number" ;
  .

bf:Isbn
  a owl:Class ;
  rdfs:subClassOf bf:Identifier ;
  rdfs:label "ISBN" ;
  dcterms:modified "2016-04-21 (New)" ;
  skos:definition "International Standard Book Number" ;
  .

bf:Ismn
  a owl:Class ;
  rdfs:subClassOf bf:Identifier ;
  rdfs:label "ISMN" ;
  dcterms:modified "2016-04-21 (New)" ;
  skos:definition "International Standard Music Number" ;
  .

bf:Isni
  a owl:Class ;
  rdfs:subClassOf bf:Identifier ;
  rdfs:label "ISNI" ;
  dcterms:modified "2017-02-03 (New)" ;
  skos:definition "International Standard Name Identifier, a unique, persistent reference number for the identities of contributors to creative works" ;
  .

bf:Iso
  a owl:Class ;
  rdfs:subClassOf bf:Identifier ;
  rdfs:label "ISO number" ;
  dcterms:modified "2016-04-21 (New)" ;
  skos:definition "International Organization for Standardization standard number" ;
  .

bf:Isrc
  a owl:Class ;
  rdfs:subClassOf bf:Identifier ;
  rdfs:label "ISRC" ;
  dcterms:modified "2016-04-21 (New)" ;
  skos:definition "International Standard Recording Code" ;
  .

bf:Issn
  a owl:Class ;
  rdfs:subClassOf bf:Identifier ;
  rdfs:label "ISSN" ;
  dcterms:modified "2016-04-21 (New)" ;
  skos:definition "International Standard Serial Number" ;
  .

bf:IssnL
  a owl:Class ;
  rdfs:subClassOf bf:Identifier ;
  rdfs:label "ISSN-L" ;
  dcterms:modified "2016-04-21 (New)" ;
  skos:definition "International Standard Serial Number that links together various media versions of a continuing resource" ;
  .

bf:Issuance
  a owl:Class ;
  rdfs:label "Mode of issuance" ;
  dcterms:modified "2016-04-21 (New)" ;
  skos:definition "Information about whether a resource is issued in one or more parts, the way it is updated, and its intended termination" ;
  .

bf:Istc
  a owl:Class ;
  rdfs:subClassOf bf:Identifier ;
  rdfs:label "ISTC" ;
  dcterms:modified "2016-04-21 (New)" ;
  skos:definition "International Standard Text Code, a numbering system developed to enable the unique identification of textual works" ;
  .

bf:Iswc
  a owl:Class ;
  rdfs:subClassOf bf:Identifier ;
  rdfs:label "ISWC" ;
  dcterms:modified "2016-04-21 (New)" ;
  skos:definition "International Standard Musical Work Code, a unique, persistent reference number for the identification of musical works" ;
  .

bf:Item
  a owl:Class ;
  rdfs:label "Item" ;
  dcterms:modified "2016-04-21 (New)" ;
  skos:definition "Single example of an Instance" ;
  .

bf:Jurisdiction
  a owl:Class ;
  rdfs:subClassOf bf:Agent ;
  rdfs:label "Jurisdiction" ;
  dcterms:modified "2016-04-21 (New)" ;
  skos:definition "Legal or political unit administering a geographic area" ;
  .

bf:KeyTitle
  a owl:Class ;
  rdfs:subClassOf bf:VariantTitle ;
  rdfs:label "Key title" ;
  dcterms:modified "2016-04-21 (New)" ;
  skos:definition "Unique title for a continuing resource that is assigned by the ISSN International Center in conjunction with an ISSN" ;
  .

bf:Kit
  a owl:Class ;
  rdfs:subClassOf bf:MixedMaterial ;
  rdfs:label "Kit" ;
  dcterms:modified "2022-10-03 (New [GH91])" ;
  skos:definition "Resource that contains a mixture of various components issued as a unit and intended primarily for instructional purposes" ;
  .

bf:Language
  a owl:Class ;
  rdfs:label "Language entity" ;
  dcterms:modified "2016-04-21 (New)" ;
  skos:definition "Language entity" ;
  .

bf:Layout
  a owl:Class ;
  rdfs:label "Layout" ;
  dcterms:modified "2016-04-21 (New)" ;
  skos:definition "Arrangement of text, images, tactile notation, etc., in a resource" ;
  .

bf:LcOverseasAcq
  a owl:Class ;
  rdfs:subClassOf bf:Identifier ;
  rdfs:label "LC acquisition program" ;
  dcterms:modified "2016-04-21 (New)" ;
  skos:definition "Identification number assigned by the Library of Congress to works acquired through one of its collaborative overseas acquisition programs" ;
  .

bf:Lccn
  a owl:Class ;
  rdfs:subClassOf bf:Identifier ;
  rdfs:label "LCCN" ;
  dcterms:modified "2016-04-21 (New)" ;
  skos:definition "Library of Congress Control Number that identifies a resource description" ;
  .

bf:Local
  a owl:Class ;
  rdfs:subClassOf bf:Identifier ;
  rdfs:label "Local identifier" ;
  dcterms:modified "2016-04-21 (New)" ;
  skos:definition "Identifier established locally and not a standard number" ;
  .

bf:Manufacture
  a owl:Class ;
  rdfs:subClassOf bf:ProvisionActivity ;
  rdfs:label "Manufacturer" ;
  dcterms:modified "2016-04-21 (New)" ;
  skos:definition "Information relating to manufacture of a resource" ;
  .

bf:Manuscript
  a owl:Class ;
  rdfs:subClassOf bf:Work ;
  rdfs:label "Manuscript" ;
  dcterms:modified
    "2016-04-21 (New)" ,
    "2022-10-03 (changed subClassOf [GH92])"
    ;
  skos:definition "Resource which is written in handwriting or typescript" ;
  .

bf:Material
  a owl:Class ;
  rdfs:label "Material" ;
  dcterms:modified "2021-06-09 (New [GH28])" ;
  skos:definition "Substance or composition of the resource" ;
  .

bf:MatrixNumber
  a owl:Class ;
  rdfs:subClassOf bf:Identifier ;
  rdfs:label "Audio matrix number" ;
  dcterms:modified
    "2016-04-21 (New)" ,
    "2017-02-03 (Revised definition)"
    ;
  skos:definition "Matrix identifier assigned to the master from which a specific sound recording was pressed" ;
  .

bf:Media
  a owl:Class ;
  rdfs:label "Media type" ;
  dcterms:modified "2016-04-21 (New)" ;
  skos:definition "Categorization reflecting the general type of intermediation device required to view, play, run, etc., the content of a resource" ;
  .

bf:Meeting
  a owl:Class ;
  rdfs:subClassOf bf:Agent ;
  rdfs:label "Meeting" ;
  dcterms:modified "2016-04-21 (New)" ;
  skos:definition "Gathering of individuals or representatives of various bodies for the purpose of discussing and/or acting on topics of common interest" ;
  .

bf:Microform
  a owl:Class ;
  rdfs:subClassOf bf:Instance ;
  rdfs:label "Microform" ;
  dcterms:modified "2023-11-30 (New [GH101])" ;
  skos:definition "Resource that contains microimages, either transparent or opaque, that may be reproductions of existing textual or graphic materials or may be original publications" ;
  .

bf:MixedMaterial
  a owl:Class ;
  rdfs:subClassOf bf:Work ;
  rdfs:label "Mixed material" ;
  dcterms:modified
    "2016-04-21 (New)" ,
    "2022-10-03 (revised definition [GH92])"
    ;
  skos:definition "Resource comprised of multiple types which is not driven by software, e.g. an archival collection of text, photographs and sound recordings" ;
  .

bf:Modification
  a owl:Class ;
  rdfs:subClassOf bf:ProvisionActivity ;
  rdfs:label "Modification" ;
  dcterms:modified "2022-10-03 (New [GH69])" ;
  skos:definition "Information relating to modification of a resource" ;
  .

bf:Monograph
  a owl:Class ;
  rdfs:subClassOf bf:Work ;
  rdfs:label "Monograph" ;
  dcterms:modified "2022-10-03 (New [GH91])" ;
  skos:definition "Resource that is issued as a single physical unit or intangible single logical unit" ;
  .

bf:Mount
  a owl:Class ;
  rdfs:label "Mount" ;
  dcterms:modified
    "2016-04-21 (New)" ,
    "2021-06-09 (Amended definition [GH29])"
    ;
  skos:definition "Physical material or object used for the support or backing to which the base material of a resource has been attached" ;
  .

bf:MovementNotation
  a owl:Class ;
  rdfs:subClassOf bf:Notation ;
  rdfs:label "Movement notation" ;
  dcterms:modified
    "2016-04-21 (New)" ,
    "2021-06-09 (Modified label [GH67])"
    ;
  skos:definition "Information on the symbol system used to convey the content of a movement resource" ;
  .

bf:MovingImage
  a owl:Class ;
  rdfs:subClassOf bf:Work ;
  rdfs:label "Moving image" ;
  dcterms:modified
    "2016-04-21 (New)" ,
    "2016-04-26 (fixed typo in definition)"
    ;
  skos:definition "Images intended to be perceived as moving, including motion pictures (using live action and/or animation) or video recordings of performances or events" ;
  .

bf:Multimedia
  a owl:Class ;
  rdfs:subClassOf bf:Work ;
  rdfs:label "Software or multimedia" ;
  dcterms:modified
    "2016-04-21 (New)" ,
    "2022-10-03 (revised definition [GH92])"
    ;
  skos:definition "Electronic resource which is a computer program or consists of multiple media types that are software driven, such as videogames" ;
  .

bf:MusicAudio
  a owl:Class ;
  rdfs:subClassOf bf:Audio ;
  rdfs:label "Music audio" ;
  dcterms:modified "2022-10-03 (New [GH91])" ;
  skos:definition "Music resource expressed in an audible form" ;
  .

bf:MusicDistributorNumber
  a owl:Class ;
  rdfs:subClassOf bf:Identifier ;
  rdfs:label "Music distributor number" ;
  dcterms:modified "2017-02-07 (New)" ;
  skos:definition "Identifier appearing on a resource assigned by a distributor to a specific audio recording, notated music publication, music-related publication, or videorecording" ;
  .

bf:MusicEnsemble
  a owl:Class ;
  rdfs:subClassOf bf:Ensemble ;
  rdfs:label "Music ensemble" ;
  dcterms:modified
    "2016-04-21 (New)" ,
    "2021-06-09 (Changed subclass to Ensemble [GH56])"
    ;
  skos:definition "Ensemble for which a musical work is appropriate" ;
  .

bf:MusicFormat
  a owl:Class ;
  rdfs:label "Notated music format" ;
  dcterms:modified "2016-04-21 (New)" ;
  skos:definition "Layout for content of a resource that is presented in the form of musical notation" ;
  .

bf:MusicInstrument
  a owl:Class ;
  rdfs:label "Musical instrument" ;
  dcterms:modified "2016-04-21 (New)" ;
  skos:definition "Instrument for which a musical work is appropriate" ;
  .

bf:MusicMedium
  a owl:Class ;
  rdfs:label "Music medium information" ;
  dcterms:modified "2016-04-21 (New)" ;
  skos:definition "Summary statement of the medium for a musical work" ;
  .

bf:MusicNotation
  a owl:Class ;
  rdfs:subClassOf bf:Notation ;
  rdfs:label "Music notation" ;
  dcterms:modified
    "2016-04-21 (New)" ,
    "2021-06-09 (Modified label [GH67])"
    ;
  skos:definition "Information on the symbol system used to convey the content of a music resource" ;
  .

bf:MusicPlate
  a owl:Class ;
  rdfs:subClassOf bf:Identifier ;
  rdfs:label "Music plate number" ;
  dcterms:modified
    "2016-04-21 (New)" ,
    "2017-02-03 (Revised definition)"
    ;
  skos:definition "Identifiers assigned by a music publisher or printer to the printing plates for the notated portion of a notated music publication, or an identifier that emulates the printing plate tradition in contemporary publications" ;
  .

bf:MusicPublisherNumber
  a owl:Class ;
  rdfs:subClassOf bf:Identifier ;
  rdfs:label "Music publisher number" ;
  dcterms:modified
    "2016-04-21 (New)" ,
    "2017-02-03 (Revised definition)"
    ;
  skos:definition "Identifier assigned to a notated music publication other than an issue, matrix, or plate number" ;
  .

bf:MusicVoice
  a owl:Class ;
  rdfs:label "Music voice" ;
  dcterms:modified "2016-04-21 (New)" ;
  skos:definition "Voice for which a musical work is appropriate" ;
  .

bf:Nbn
  a owl:Class ;
  rdfs:subClassOf bf:Identifier ;
  rdfs:label "NBN" ;
  dcterms:modified "2016-04-21 (New)" ;
  skos:definition "National Bibliography Number that identifies a resource description" ;
  .

bf:NonMusicAudio
  a owl:Class ;
  rdfs:subClassOf bf:Audio ;
  rdfs:label "Non-music audio" ;
  dcterms:modified "2022-10-03 (New [GH91])" ;
  skos:definition "Resource expressed in an audible form, including spoken word and other non-musical sounds" ;
  .

bf:NotatedMovement
  a owl:Class ;
  rdfs:subClassOf bf:Work ;
  rdfs:label "Notated movement" ;
  dcterms:modified "2016-04-21 (New)" ;
  skos:definition "Graphic, non-realized representations of movement intended to be perceived visually, e.g. dance" ;
  .

bf:NotatedMusic
  a owl:Class ;
  rdfs:subClassOf bf:Work ;
  rdfs:label "Notated music" ;
  dcterms:modified "2016-04-21 (New)" ;
  skos:definition "Graphic, non-realized representations of musical works intended to be perceived visually" ;
  .

bf:Notation
  a owl:Class ;
  rdfs:label "Notation" ;
  dcterms:modified "2016-04-21 (New)" ;
  skos:definition "Information on the alphabet, script, or symbol system used to convey the content of the resource, including specialized scripts, typefaces, tactile notation, movement notation, and musical notation" ;
  .

bf:Note
  a owl:Class ;
  rdfs:label "Note" ;
  dcterms:modified
    "2016-04-21 (New)" ,
    "2021-06-09 (Added editorial note [GH35])"
    ;
  skos:definition "Information, usually in textual form, on attributes of a resource or some aspect of a resource" ;
  skos:editorialNote "Any entry from the Note Types vocabulary at ID may be used; all have been defined as a bf:Note" ;
  .

bf:Object
  a owl:Class ;
  rdfs:subClassOf bf:Work ;
  rdfs:label "Three-dimensional object" ;
  dcterms:modified "2016-04-21 (New)" ;
  skos:definition "Resource in a form intended to be perceived visually in three-dimensions, including man-made objects such as models, sculptures, clothing, and toys, as well as naturally occurring objects such as specimens mounted for viewing" ;
  .

bf:ObjectCount
  a owl:Class ;
  rdfs:subClassOf bf:DigitalCharacteristic ;
  rdfs:label "Digital cartographic object count" ;
  dcterms:modified "2016-04-21 (New)" ;
  skos:definition "Number of objects in encoded geospatial information in a cartographic resource" ;
  .

bf:OclcNumber
  a owl:Class ;
  rdfs:subClassOf bf:Identifier ;
  rdfs:label "OCLC number" ;
  dcterms:modified "2024-07-10 (New [GH120])" ;
  skos:definition "Identifier assigned by OCLC" ;
  .

bf:Organization
  a owl:Class ;
  rdfs:subClassOf bf:Agent ;
  rdfs:label "Organization" ;
  dcterms:modified "2016-04-21 (New)" ;
  skos:definition "Corporation or group of persons and/or organizations that acts, or may act, as a unit" ;
  .

bf:ParallelTitle
  a owl:Class ;
  rdfs:subClassOf bf:VariantTitle ;
  rdfs:label "Parallel title proper" ;
  dcterms:modified "2016-04-21 (New)" ;
  skos:definition "Title in another language and/or script" ;
  .

bf:Person
  a owl:Class ;
  rdfs:subClassOf
    bf:Agent ,
    foaf:Person
    ;
  rdfs:label "Person" ;
  dcterms:modified "2016-04-21 (New)" ;
  skos:definition "Individual or identity established by an individual (either alone or in collaboration with one or more other individuals)" ;
  .

bf:Place
  a owl:Class ;
  rdfs:label "Place" ;
  dcterms:modified "2016-04-21 (New)" ;
  skos:definition "Geographic location" ;
  .

bf:PlaybackChannels
  a owl:Class ;
  rdfs:subClassOf bf:SoundCharacteristic ;
  rdfs:label "Configuration of playback channels" ;
  dcterms:modified "2016-04-21 (New)" ;
  skos:definition "Configuration/number of sound channels used to make a recording, such as one channel for a monophonic recording, e.g., mono, stereo, quadraphonic, surround" ;
  .

bf:PlaybackCharacteristic
  a owl:Class ;
  rdfs:subClassOf bf:SoundCharacteristic ;
  rdfs:label "Special playback characteristics" ;
  dcterms:modified "2016-04-21 (New)" ;
  skos:definition "Equalization system, noise reduction system, etc., used in making an audio recording, e.g., CCIR standard, CX encoded, Dolby" ;
  .

bf:PlayingSpeed
  a owl:Class ;
  rdfs:subClassOf bf:SoundCharacteristic ;
  rdfs:label "Playing speed" ;
  dcterms:modified "2016-04-21 (New)" ;
  skos:definition "Speed at which an audio carrier must be operated to produce the sound intended, e.g., 78 rpm, 19 cm/s" ;
  .

bf:Polarity
  a owl:Class ;
  rdfs:label "Polarity" ;
  dcterms:modified "2016-04-21 (New)" ;
  skos:definition "Relationship of the colors and tones in an image to the colors and tones of the object reproduced" ;
  .

bf:PostalRegistration
  a owl:Class ;
  rdfs:subClassOf bf:Identifier ;
  rdfs:label "Postal registration number" ;
  dcterms:modified "2016-04-21 (New)" ;
  skos:definition "Number assigned to a publication for which the specified postal service permits the use of a special mailing class privilege" ;
  .

bf:PresentationFormat
  a owl:Class ;
  rdfs:subClassOf bf:ProjectionCharacteristic ;
  rdfs:label "Presentation format" ;
  dcterms:modified "2016-04-21 (New)" ;
  skos:definition "Format used in the production of a projected image, e.g., Cinerama, IMAX" ;
  .

bf:PrimaryContribution
  a owl:Class ;
  rdfs:subClassOf bf:Contribution ;
  rdfs:label "Primary contribution" ;
  dcterms:modified "2023-11-30 (New [GH104])" ;
  skos:definition "Contribution for which the agent is the name chosen as the name part of the name and title access point" ;
  .

bf:Print
  a owl:Class ;
  rdfs:subClassOf bf:Instance ;
  rdfs:label "Printed" ;
  dcterms:modified "2016-04-21 (New)" ;
  skos:definition "Resource that is printed" ;
  .

bf:Production
  a owl:Class ;
  rdfs:subClassOf bf:ProvisionActivity ;
  rdfs:label "Producer" ;
  dcterms:modified "2016-04-21 (New)" ;
  skos:definition "Information relating to production of a resource" ;
  .

bf:ProductionMethod
  a owl:Class ;
  rdfs:label "Production method" ;
  dcterms:modified "2016-04-21 (New)" ;
  skos:definition "Process used to produce a resource" ;
  .

bf:Projection
  a owl:Class ;
  rdfs:label "Projection" ;
  dcterms:modified "2017-02-03 (New)" ;
  skos:definition "Method or system used to represent the surface of the earth or of a celestial sphere on a plane" ;
  .

bf:ProjectionCharacteristic
  a owl:Class ;
  rdfs:label "Projection characteristic" ;
  dcterms:modified "2016-04-21 (New)" ;
  skos:definition "Technical specification relating to the projection of a motion picture film" ;
  .

bf:ProjectionSpeed
  a owl:Class ;
  rdfs:subClassOf bf:ProjectionCharacteristic ;
  rdfs:label "Projection speed" ;
  dcterms:modified "2016-04-21 (New)" ;
  skos:definition "Speed at which a projected carrier must be operated to produce the moving image intended, e.g., 20 fps" ;
  .

bf:ProvisionActivity
  a owl:Class ;
  rdfs:label "Provider entity" ;
  dcterms:modified "2016-04-21 (New)" ;
  skos:definition "Information about the agent or place relating to the publication, printing, distribution, issue, release, or production of a resource" ;
  .

bf:PubFrequency
  a owl:Class ;
  rdfs:label "Publication Frequency" ;
  dcterms:modified "2021-06-09 (New [GH76])" ;
  skos:definition "Information about the publication frequency of a resource" ;
  .

bf:Publication
  a owl:Class ;
  rdfs:subClassOf bf:ProvisionActivity ;
  rdfs:label "Publisher" ;
  dcterms:modified "2016-04-21 (New)" ;
  skos:definition "Information relating to publication of a resource" ;
  .

bf:PublisherNumber
  a owl:Class ;
  rdfs:subClassOf bf:Identifier ;
  rdfs:label "Publisher number" ;
  dcterms:modified "2016-04-21 (New)" ;
  skos:definition "Number assigned by a publisher that is not one of the specific defined types" ;
  .

bf:RecordingMedium
  a owl:Class ;
  rdfs:subClassOf bf:SoundCharacteristic ;
  rdfs:label "Recording medium" ;
  dcterms:modified "2016-04-21 (New)" ;
  skos:definition "Type of medium used to record sound on an audio carrier, e.g., magnetic, optical" ;
  .

bf:RecordingMethod
  a owl:Class ;
  rdfs:subClassOf bf:SoundCharacteristic ;
  rdfs:label "Type of recording" ;
  dcterms:modified "2016-04-21 (New)" ;
  skos:definition "Method used to encode audio content for playback, e.g., analog, digital" ;
  .

bf:ReductionRatio
  a owl:Class ;
  rdfs:label "Reduction ratio" ;
  dcterms:modified "2016-04-21 (New)" ;
  skos:definition "Size of a micro-image in relation to the original from which it was produced" ;
  .

bf:RegionalEncoding
  a owl:Class ;
  rdfs:subClassOf bf:DigitalCharacteristic ;
  rdfs:label "Regional encoding" ;
  dcterms:modified "2016-04-21 (New)" ;
  skos:definition "Identification of the region of the world for which a videodisc has been encoded, e.g., region 4" ;
  .

bf:Relation
  a owl:Class ;
  rdfs:label "Relation" ;
  dcterms:modified "2024-07-10 (New [GH116])" ;
  skos:definition "Associated resource and its relationship to the resource being described" ;
  .

bf:Relationship
  a owl:Class ;
  rdfs:label "Relationship" ;
  dcterms:modified "2024-07-10 (New [GH116])" ;
  skos:definition "Type of relationship between resources" ;
  .

bf:Relief
  a owl:Class ;
  rdfs:label "Relief" ;
  dcterms:modified "2023-11-30 (New [GH104])" ;
  skos:definition "Relief term specified on a cartographic resource" ;
  .

bf:ReportNumber
  a owl:Class ;
  rdfs:subClassOf bf:Identifier ;
  rdfs:label "Technical report number" ;
  dcterms:modified "2016-04-21 (New)" ;
  skos:definition "Identification number of a technical report that is not a Standard Technical Report Number" ;
  .

bf:Resolution
  a owl:Class ;
  rdfs:subClassOf bf:DigitalCharacteristic ;
  rdfs:label "Resolution" ;
  dcterms:modified "2016-04-21 (New)" ;
  skos:definition "Clarity or fineness of detail in a digital image, expressed by the measurement of the image in pixels, etc., e.g., 3.1 megapixels" ;
  .

bf:RetentionPolicy
  a owl:Class ;
  rdfs:subClassOf bf:UsageAndAccessPolicy ;
  rdfs:label "Retention policy" ;
  dcterms:modified "2016-04-21 (New)" ;
  skos:definition "Policy of holding institution for retaining resource" ;
  .

bf:Review
  a owl:Class ;
  rdfs:label "Review" ;
  dcterms:modified "2016-04-21 (New)" ;
  skos:definition "Review of a resource" ;
  .

bf:Role
  a owl:Class ;
  rdfs:label "Role" ;
  dcterms:modified "2017-02-03 (New)" ;
  skos:definition "Function played or provided by a contributor, e.g., author or illustrator" ;
  .

bf:Scale
  a owl:Class ;
  rdfs:label "Scale" ;
  dcterms:modified "2017-02-03 (New)" ;
  skos:definition "Ratio of the dimensions of a form contained or embodied in a resource to the dimensions of the entity it represents, e.g., for images or cartographic resources" ;
  .

bf:Script
  a owl:Class ;
  rdfs:subClassOf bf:Notation ;
  rdfs:label "Script" ;
  dcterms:modified
    "2016-04-21 (New)" ,
    "2021-06-09 (Modified label [GH67])"
    ;
  skos:definition "Information on the script, or symbol system used to convey the content of a text resource" ;
  .

bf:Serial
  a owl:Class ;
  rdfs:subClassOf bf:Work ;
  rdfs:label "Serial" ;
  dcterms:modified "2022-10-03 (New [GH91])" ;
  skos:definition "Resource that is issued in successive parts, usually numbered, that has no predetermined conclusion" ;
  .

bf:Series
  a owl:Class ;
  rdfs:subClassOf bf:Work ;
  rdfs:label "Series" ;
  dcterms:modified "2022-10-03 (New [GH91])" ;
  skos:definition "Resource with a collective title that applies to a group of separate resources, each of which also has its own title" ;
  .

bf:ShelfMark
  a owl:Class ;
  rdfs:subClassOf bf:Identifier ;
  rdfs:label "Shelf location" ;
  dcterms:modified "2016-04-21 (New)" ;
  skos:definition "Piece/item identifier, such as a call or other type of number" ;
  .

bf:ShelfMarkDdc
  a owl:Class ;
  rdfs:subClassOf bf:ShelfMark ;
  rdfs:label "DDC call number" ;
  dcterms:modified "2016-04-21 (New)" ;
  skos:definition "Shelf mark based on Dewey Decimal Classification" ;
  .

bf:ShelfMarkLcc
  a owl:Class ;
  rdfs:subClassOf bf:ShelfMark ;
  rdfs:label "LCC call number" ;
  dcterms:modified "2016-04-21 (New)" ;
  skos:definition "Shelf mark based on Library of Congress Classification" ;
  .

bf:ShelfMarkNlm
  a owl:Class ;
  rdfs:subClassOf bf:ShelfMark ;
  rdfs:label "NLM call number" ;
  dcterms:modified "2016-04-21 (New)" ;
  skos:definition "Shelf mark based on National Library of Medicine Classification" ;
  .

bf:ShelfMarkUdc
  a owl:Class ;
  rdfs:subClassOf bf:ShelfMark ;
  rdfs:label "UDC call number" ;
  dcterms:modified "2016-04-21 (New)" ;
  skos:definition "Shelf mark based on Universal Decimal Classification" ;
  .

bf:Sici
  a owl:Class ;
  rdfs:subClassOf bf:Identifier ;
  rdfs:label "SICI" ;
  dcterms:modified "2016-04-21 (New)" ;
  skos:definition "Serial Item and Contribution Identifier" ;
  .

bf:SoundCharacteristic
  a owl:Class ;
  rdfs:label "Sound characteristic" ;
  dcterms:modified "2016-04-21 (New)" ;
  skos:definition "Technical specification relating to the encoding of sound in a resource" ;
  .

bf:SoundContent
  a owl:Class ;
  rdfs:label "Sound content" ;
  dcterms:modified "2016-04-21 (New)" ;
  skos:definition "Indication of whether the production of sound is an integral part of the resource" ;
  .

bf:Source
  a owl:Class ;
  rdfs:label "Source" ;
  dcterms:modified "2016-04-21 (New)" ;
  skos:definition "Resource from which value or label came or was derived" ;
  .

bf:Status
  a owl:Class ;
  rdfs:label "Status" ;
  dcterms:modified "2016-04-21 (New)" ;
  skos:definition "Designation of the validity or position of something, e.g., whether something is incorrect or available" ;
  .

bf:StillImage
  a owl:Class ;
  rdfs:subClassOf bf:Work ;
  rdfs:label "Still image" ;
  dcterms:modified "2016-04-21 (New)" ;
  skos:definition "Resource expressed through line, shape, shading, etc., intended to be perceived visually as a still image or images in two dimensions, including two-dimensional images and slides and transparencies" ;
  .

bf:StockNumber
  a owl:Class ;
  rdfs:subClassOf bf:Identifier ;
  rdfs:label "Stock number" ;
  dcterms:modified "2016-04-21 (New)" ;
  skos:definition "Identification number used for stock purposes and assigned by agencies such as distributors, publishers, or vendors" ;
  .

bf:Strn
  a owl:Class ;
  rdfs:subClassOf bf:Identifier ;
  rdfs:label "STRN" ;
  dcterms:modified "2016-04-21 (New)" ;
  skos:definition "Standard Technical Report Number" ;
  .

bf:StudyNumber
  a owl:Class ;
  rdfs:subClassOf bf:Identifier ;
  rdfs:label "Study number" ;
  dcterms:modified "2016-04-21 (New)" ;
  skos:definition "Identification number for a computer data file" ;
  .

bf:Sublocation
  a owl:Class ;
  rdfs:label "Sublocation" ;
  dcterms:modified "2016-04-21 (New)" ;
  skos:definition "Specific place within the holding entity where the item is located or made available" ;
  .

bf:Summary
  a owl:Class ;
  rdfs:label "Summary" ;
  dcterms:modified "2016-04-21 (New)" ;
  skos:definition "Description of the content of a resource, such as an abstract, summary, etc." ;
  .

bf:SupplementaryContent
  a owl:Class ;
  rdfs:label "Supplementary material" ;
  dcterms:modified "2016-04-21 (New)" ;
  skos:definition "Index, bibliography, appendix, etc. intended to supplement the primary content of a resource" ;
  .

bf:SystemRequirement
  a owl:Class ;
  rdfs:label "System Requirement" ;
  dcterms:modified "2017-02-06 (New)" ;
  skos:definition "Equipment or system requirements beyond what is normal and obvious for the type of carrier or type of file, such as make and model of equipment or hardware, operating system, amount of memory, programming language, other necessary software, any plug-ins or peripherals required to play, view, or run the resource" ;
  .

bf:TableOfContents
  a owl:Class ;
  rdfs:label "Table of contents" ;
  dcterms:modified "2016-04-21 (New)" ;
  skos:definition "Table of contents of a resource" ;
  .

bf:Tactile
  a owl:Class ;
  rdfs:subClassOf bf:Instance ;
  rdfs:label "Tactile material" ;
  dcterms:modified "2016-04-21 (New)" ;
  skos:definition "Resource that is intended to be perceived by touch" ;
  .

bf:TactileNotation
  a owl:Class ;
  rdfs:subClassOf bf:Notation ;
  rdfs:label "Tactile notation" ;
  dcterms:modified
    "2016-04-21 (New)" ,
    "2021-06-09 (Modified label [GH67])"
    ;
  skos:definition "Information on the symbol system used to convey the content of a tactile resource" ;
  .

bf:TapeConfig
  a owl:Class ;
  rdfs:subClassOf bf:SoundCharacteristic ;
  rdfs:label "Tape configuration" ;
  dcterms:modified "2016-04-21 (New)" ;
  skos:definition "Number of tracks on an audiotape, e.g., 12 track" ;
  .

bf:Temporal
  a owl:Class ;
  rdfs:label "Temporal concept" ;
  dcterms:modified "2016-04-21 (New)" ;
  skos:definition "Chronological period" ;
  .

bf:Text
  a owl:Class ;
  rdfs:subClassOf bf:Work ;
  rdfs:label "Text" ;
  dcterms:modified "2016-04-21 (New)" ;
  skos:definition "Resource intended to be perceived visually and understood through the use of language in written or spoken form" ;
  .

bf:Title
  a owl:Class ;
  rdfs:label "Title entity" ;
  dcterms:modified
    "2016-04-21 (New)" ,
    "2017-02-03 (Definition changed)"
    ;
  skos:definition "Title information relating to a resource: work title, preferred title, instance title, transcribed title, translated title, variant form of title, etc." ;
  .

bf:Topic
  a owl:Class ;
  rdfs:label "Topic" ;
  dcterms:modified "2016-04-21 (New)" ;
  skos:definition "Concept or area of knowledge" ;
  .

bf:TrackConfig
  a owl:Class ;
  rdfs:subClassOf bf:SoundCharacteristic ;
  rdfs:label "Track configuration" ;
  dcterms:modified "2016-04-21 (New)" ;
  skos:definition "Configuration of the audio track on a sound-track film, e.g., center track, edge track" ;
  .

bf:TransliteratedTitle
  a owl:Class ;
  rdfs:subClassOf bf:VariantTitle ;
  rdfs:label "Transliterated title" ;
  dcterms:modified "2023-11-30 (New [GH104])" ;
  skos:definition "Title transliterated from one script to another" ;
  .

bf:Unit
  a owl:Class ;
  rdfs:label "Unit" ;
  dcterms:modified "2016-04-21 (New)" ;
  skos:definition "Units in which a value is expressed" ;
  .

bf:Upc
  a owl:Class ;
  rdfs:subClassOf bf:Identifier ;
  rdfs:label "UPC" ;
  dcterms:modified "2016-04-21 (New)" ;
  skos:definition "Universal Product Code" ;
  .

bf:Urn
  a owl:Class ;
  rdfs:subClassOf bf:Identifier ;
  rdfs:label "URN" ;
  dcterms:modified
    "2016-04-21 (New)" ,
    "2021-06-09 (Corrected definition [GH51])"
    ;
  skos:definition "Uniform Resource Name" ;
  .

bf:UsageAndAccessPolicy
  a owl:Class ;
  rdfs:label "Use and access conditions" ;
  dcterms:modified "2016-04-21 (New)" ;
  skos:definition "General statement of allowances and restrictions on access to a resource, including retention, reproduction, access, and lending" ;
  .

bf:UsePolicy
  a owl:Class ;
  rdfs:subClassOf bf:UsageAndAccessPolicy ;
  rdfs:label "Use policy" ;
  dcterms:modified "2016-04-21 (New)" ;
  skos:definition "Usage limitations placed on a resource with respect to reproduction, publication, exhibition, etc." ;
  .

bf:VariantTitle
  a owl:Class ;
  rdfs:subClassOf bf:Title ;
  rdfs:label "Title variation" ;
  dcterms:modified "2016-04-21 (New)" ;
  skos:definition "Title associated with the resource that is different from the Work or Instance title" ;
  .

bf:VideoCharacteristic
  a owl:Class ;
  rdfs:label "Video characteristic" ;
  dcterms:modified "2016-04-21 (New)" ;
  skos:definition "Technical specification relating to the encoding of video images in a resource" ;
  .

bf:VideoFormat
  a owl:Class ;
  rdfs:subClassOf bf:VideoCharacteristic ;
  rdfs:label "Video format" ;
  dcterms:modified "2016-04-21 (New)" ;
  skos:definition "Standard, etc., used to encode the analog video content of a resource, e.g., Beta, 8mm" ;
  .

bf:VideoRecordingNumber
  a owl:Class ;
  rdfs:subClassOf bf:Identifier ;
  rdfs:label "Video recording number" ;
  dcterms:modified
    "2016-04-21 (New)" ,
    "2017-02-03 (Corrected case in class name)"
    ;
  skos:definition "Number assigned by a publisher to a video recording" ;
  .

bf:Work
  a owl:Class ;
  rdfs:label "Work" ;
  dcterms:modified "2016-04-21 (New)" ;
  skos:definition "Resource reflecting a conceptual essence of a cataloging resource" ;
  .

bf:absorbed
  a owl:ObjectProperty ;
  rdfs:subPropertyOf bf:precededBy ;
  rdfs:label "Absorption of" ;
  rdfs:comment
    "Suggested use - With Work or Instance" ,
    "Suggested value - Work or Instance"
    ;
  dcterms:modified
    "2016-04-21 (New)" ,
    "2016-04-29 (added inverse, updated range)"
    ;
  owl:inverseOf bf:absorbedBy ;
  skos:definition "Resource that has been incorporated into another resource" ;
  .

bf:absorbedBy
  a owl:ObjectProperty ;
  rdfs:subPropertyOf bf:succeededBy ;
  rdfs:label "Absorbed by" ;
  rdfs:comment
    "Suggested use - With Work or Instance" ,
    "Suggested value - Work or Instance"
    ;
  dcterms:modified
    "2016-04-21 (New)" ,
    "2016-04-29 (added inverse, updated range)"
    ;
  owl:inverseOf bf:absorbed ;
  skos:definition "Resource that incorporates another resource" ;
  .

bf:accompaniedBy
  a owl:ObjectProperty ;
  rdfs:subPropertyOf bf:relatedTo ;
  rdfs:label "Accompanied by" ;
  rdfs:comment
    "Suggested use - With Work, Instance or Item" ,
    "Suggested value - Work, Instance or Item"
    ;
  dcterms:modified
    "2016-04-21 (New)" ,
    "2016-04-29 (added inverse)"
    ;
  owl:inverseOf bf:accompanies ;
  skos:definition "Resource that accompanies the described resource" ;
  .

bf:accompanies
  a owl:ObjectProperty ;
  rdfs:subPropertyOf bf:relatedTo ;
  rdfs:label "Accompanies" ;
  rdfs:comment
    "Suggested use - With Work, Instance or Item" ,
    "Suggested value - Work, Instance or Item"
    ;
  dcterms:modified
    "2016-04-21 (New)" ,
    "2016-04-29 (added inverse)"
    ;
  owl:inverseOf bf:accompaniedBy ;
  skos:definition "Resource that adds to or is issued with the described resource" ;
  .

bf:acquisitionSource
  a owl:ObjectProperty ;
  rdfs:label "Source of acquisition" ;
  rdfs:comment "Suggested use - With Work or Instance" ;
  dcterms:modified
    "2016-04-21 (New)" ,
    "2017-02-06 (Changed from data to object property, slight change to definition)" ,
    "2021-06-09 (Broadened range [GH63])" ,
    "2025-01-23 (Ontological correction - partially addresses [GH121])"
    ;
  skos:definition "Information about an organization, person, etc., from which a resource may be obtained." ;
  .

bf:acquisitionTerms
  a owl:DatatypeProperty ;
  rdfs:label "Terms of acquisition" ;
  rdfs:comment "Suggested use - With Work or Instance" ;
  dcterms:modified "2016-04-21 (New)" ;
  rdfs:range rdfs:Literal ;
  skos:definition "Conditions under which the publisher, distributor, etc., will normally supply a resource, e.g., price of a resource." ;
  .

bf:adminMetadata
  a owl:ObjectProperty ;
  rdfs:label "Administrative metadata" ;
  dcterms:modified
    "2016-04-21 (New)" ,
    "2025-01-23 (Ontological correction - partially addresses [GH121])"
    ;
  rdfs:range bf:AdminMetadata ;
  skos:definition "Metadata about the metadata, especially provenance information." ;
  .

bf:adminMetadataFor
  a owl:ObjectProperty ;
  rdfs:label "Administrative metadata for" ;
  dcterms:modified
    "2021-06-09 (New [GH59])" ,
    "2025-01-23 (Ontological correction - partially addresses [GH121])"
    ;
  rdfs:domain bf:AdminMetadata ;
  skos:definition "Relates an Administrative metadata resource to the resource it captures information about." ;
  .

bf:agent
  a owl:ObjectProperty ;
  rdfs:label "Associated agent" ;
  rdfs:comment "Suggested value - bf:Agent or foaf:Agent" ;
  dcterms:modified
    "2016-04-21 (New)" ,
    "2021-06-09 (Broadened range [GH63])" ,
    "2025-01-23 (Ontological correction - partially addresses [GH121])"
    ;
  skos:definition "Entity associated with a resource or element of description, such as the name of the entity responsible for the content or of the publication, printing, distribution, issue, release or production of a resource." ;
  .

bf:agentOf
  a owl:ObjectProperty ;
  rdfs:label "Associated agent of" ;
  rdfs:comment "Suggested use - With bf:Agent or foaf:Agent" ;
  dcterms:modified
    "2021-06-09 (New [GH3])" ,
    "2025-01-23 (Ontological correction - partially addresses [GH121])"
    ;
  skos:definition "Property relating an agent, such as an entity responsible for the content or of the publication, printing, distribution, issue, release or production, to another resource." ;
  .

bf:appliedMaterial
  a owl:ObjectProperty ;
  rdfs:subPropertyOf bf:material ;
  rdfs:label "Applied material" ;
  rdfs:comment "Suggested use - With Work, Instance or Item" ;
  dcterms:modified
    "2016-04-21 (New)" ,
    "2021-06-09 (Broadened range [GH24], Broadened domain, Made subproperty of material [GH26])" ,
    "2025-01-23 (Ontological correction - partially addresses [GH121])"
    ;
  skos:definition "Physical or chemical substance applied to a base material of a resource." ;
  .

bf:appliedMaterialOf
  a owl:ObjectProperty ;
  rdfs:subPropertyOf bf:materialOf ;
  rdfs:label "Appllied material of" ;
  dcterms:modified
    "2021-06-09 (New [GH25])" ,
    "2025-01-23 (Ontological correction - partially addresses [GH121])"
    ;
  rdfs:domain bf:Instance ;
  skos:definition "Relates a Material resource to that which it is the applied material of." ;
  .

bf:arrangement
  a owl:ObjectProperty ;
  rdfs:subPropertyOf bf:relatedTo ;
  rdfs:label "Arrangement" ;
  dcterms:modified
    "2016-04-21 (New)" ,
    "2021-06-09 (Redefined [GH77])"
    ;
  rdfs:domain bf:Work ;
  rdfs:range bf:Work ;
  owl:inverseOf bf:arrangementOf ;
  skos:definition "Relates one resource to another of which it is an arrangement of the first" ;
  .

bf:arrangementOf
  a owl:ObjectProperty ;
  rdfs:subPropertyOf bf:relatedTo ;
  rdfs:label "Arrangement of" ;
  dcterms:modified "2021-06-09 (New [GH77])" ;
  rdfs:domain bf:Work ;
  rdfs:range bf:Work ;
  owl:inverseOf bf:arrangement ;
  skos:definition "Relates an arrangement to the resource of which it is an arrangement." ;
  .

bf:ascensionAndDeclination
  a owl:DatatypeProperty ;
  rdfs:label "Cartographic ascension and declination" ;
  dcterms:modified "2016-04-21 (New)" ;
  rdfs:domain bf:Cartographic ;
  rdfs:range rdfs:Literal ;
  skos:definition "System for identifying the location of a celestial object in the sky covered by the cartographic content of a resource using the angles of right ascension and declination." ;
  .

bf:aspectRatio
  a owl:ObjectProperty ;
  rdfs:label "Aspect ratio" ;
  rdfs:comment "Suggested use - With Work or Instance" ;
  dcterms:modified "2016-04-21 (New)" ;
  rdfs:range bf:AspectRatio ;
  skos:definition "Proportional relationship between an image's width and its height." ;
  .

bf:assigner
  a owl:ObjectProperty ;
  rdfs:label "Assigner" ;
  rdfs:comment "Suggested value - bf:Organization or bf:Assigner" ;
  dcterms:modified
    "2016-04-21 (New)" ,
    "2021-06-09 (Broaden domain [GH60], Broadened range [GH63])" ,
    "2025-01-23 (Ontological correction - partially addresses [GH121])"
    ;
  skos:definition "Entity that assigned the metadata, such as the entity that assigned a classification number, entity that assigned a name, entity that assigned an identifier." ;
  .

bf:associatedResource
  a owl:ObjectProperty ;
  rdfs:label "Associated resource" ;
  rdfs:comment "Suggested value - With Work or Hub" ;
  dcterms:modified "2022-07-10 (New [GH116])" ;
  rdfs:domain bf:Relation ;
  skos:definition "Associated resource" ;
  .

bf:awards
  a owl:DatatypeProperty ;
  rdfs:label "Award note" ;
  rdfs:comment "Suggested use - With Work or Instance" ;
  dcterms:modified
    "2016-04-21 (New)" ,
    "2021-06-09 (Added note [GH37])"
    ;
  rdfs:range rdfs:Literal ;
  skos:definition "Information on awards associated with the described resource." ;
  skos:editorialNote "See also the ARM Ontology for strategies to model this information in greater detail." ;
  .

bf:baseMaterial
  a owl:ObjectProperty ;
  rdfs:subPropertyOf bf:material ;
  rdfs:label "Base material" ;
  rdfs:comment "Suggested use - With Work, Instance or Item" ;
  dcterms:modified
    "2016-04-21 (New)" ,
    "2021-06-09 (Broadened range [GH24], Broadened domain, Made subproperty of material [GH26])" ,
    "2025-01-23 (Ontological correction - partially addresses [GH121])"
    ;
  skos:definition "Underlying physical material of a resource." ;
  .

bf:baseMaterialOf
  a owl:ObjectProperty ;
  rdfs:subPropertyOf bf:materialOf ;
  rdfs:label "Base material of" ;
  dcterms:modified
    "2021-06-09 (New [GH25])" ,
    "2025-01-23 (Ontological correction - partially addresses [GH121])"
    ;
  rdfs:domain bf:Instance ;
  skos:definition "Relates a Material resource to that which it is the base material of." ;
  .

bf:binding
  a owl:ObjectProperty ;
  rdfs:label "Binding method" ;
  dcterms:modified
    "2022-10-03 (New [GH91])" ,
    "2025-01-23 (Ontological correction - partially addresses [GH121])"
    ;
  rdfs:domain bf:Instance ;
  skos:definition "A method used to bind a published or unpublished resource,or other binding information." ;
  .

bf:bookFormat
  a owl:ObjectProperty ;
  rdfs:label "Book format" ;
  dcterms:modified "2016-04-21 (New)" ;
  rdfs:domain bf:Instance ;
  rdfs:range bf:BookFormat ;
  skos:definition "Result of folding a printed sheet to form a gathering of leaves." ;
  .

bf:capture
  a owl:ObjectProperty ;
  rdfs:label "Capture of content" ;
  rdfs:comment "Suggested use - With Work or Instance" ;
  dcterms:modified "2016-04-21 (New)" ;
  rdfs:range bf:Capture ;
  skos:definition "Information about place and date associated with the capture (e.g., recording, filming) of the content of a resource." ;
  .

bf:carrier
  a owl:ObjectProperty ;
  rdfs:label "Carrier type" ;
  rdfs:comment "Suggested value - bf:Carrier or skos:Concept" ;
  dcterms:modified
    "2016-04-21 (New)" ,
    "2022-10-03 (Broadened range [GH72])" ,
    "2025-01-23 (Ontological correction - partially addresses [GH121])"
    ;
  rdfs:domain bf:Instance ;
  skos:definition "Categorization reflecting the format of the storage medium and housing of a carrier." ;
  .

bf:cartographicAttributes
  a owl:ObjectProperty ;
  rdfs:label "Cartographic data" ;
  rdfs:comment "Suggested use - With Work or Instance" ;
  dcterms:modified "2016-04-21 (New)" ;
  rdfs:range bf:Cartographic ;
  skos:definition "Cartographic data that identifies characteristics of the resource, such as coordinates, projection, etc." ;
  .

bf:changeDate
  a owl:DatatypeProperty ;
  rdfs:subPropertyOf bf:date ;
  rdfs:label "Description change date" ;
  dcterms:modified "2016-04-21 (New)" ;
  rdfs:domain bf:AdminMetadata ;
  rdfs:range rdfs:Literal ;
  skos:definition "Date or date and time on which the metadata was modified" ;
  .

bf:classification
  a owl:ObjectProperty ;
  rdfs:label "Classification" ;
  rdfs:comment "Suggested use - With Work, Instance or Item" ;
  dcterms:modified "2016-04-21 (New)" ;
  rdfs:range bf:Classification ;
  skos:definition "Classification number in any scheme." ;
  .

bf:classificationPortion
  a owl:DatatypeProperty ;
  rdfs:label "Classification number" ;
  dcterms:modified "2016-04-21 (New)" ;
  rdfs:domain bf:Classification ;
  rdfs:range rdfs:Literal ;
  skos:definition "Classification number (single class number or beginning number of a span) that indicates the subject by applying a formal system of coding and organizing resources." ;
  .

bf:code
  a owl:DatatypeProperty ;
  rdfs:label "Code" ;
  dcterms:modified
    "2016-04-21 (New)" ,
    "2025-01-23 (Ontological correction - partially addresses [GH121])"
    ;
  rdfs:range rdfs:Literal ;
  skos:definition "String of characters that serves as a code representing information." ;
  .

bf:collectionArrangement
  a owl:ObjectProperty ;
  rdfs:label "Collection Organization and arrangement" ;
  rdfs:comment "Suggested use - With Work or Instance" ;
  dcterms:modified "2021-06-09 (New [GH77])" ;
  rdfs:range bf:CollectionArrangement ;
  skos:definition "Information about the organization and arrangement of a collection of resources." ;
  .

bf:collectionArrangementOf
  a owl:ObjectProperty ;
  rdfs:label "Organization and arrangement of Collection" ;
  rdfs:comment "Suggested value - Work or Instance" ;
  dcterms:modified "2021-06-09 (New [GH77])" ;
  rdfs:domain bf:CollectionArrangement ;
  skos:definition "Relates an Arrangement resource to that which it describes." ;
  .

bf:collectionOrganization
  a owl:DatatypeProperty ;
  rdfs:label "Organization of material" ;
  dcterms:modified "2021-06-09 (New [GH77])" ;
  rdfs:domain bf:CollectionArrangement ;
  rdfs:range rdfs:Literal ;
  skos:definition "Manner in which the resource is divided into smaller units." ;
  .

bf:colorContent
  a owl:ObjectProperty ;
  rdfs:label "Color content" ;
  rdfs:comment "Suggested use - With Work, Instance or Item" ;
  dcterms:modified
    "2016-04-21 (New)" ,
    "2021-06-09 (Broaden range [GH31])"
    ;
  rdfs:range bf:ColorContent ;
  skos:definition "Color characteristics, e.g., black and white, multicolored." ;
  .

bf:content
  a owl:ObjectProperty ;
  rdfs:label "Content type" ;
  rdfs:comment "Suggested value - bf:Content or skos:Concept" ;
  dcterms:modified
    "2016-04-21 (New)" ,
    "2022-10-03 (Broadened range [GH71])" ,
    "2025-01-23 (Ontological correction - partially addresses [GH121])"
    ;
  rdfs:domain bf:Work ;
  skos:definition "Categorization reflecting the fundamental form of communication in which the content is expressed and the human sense through which it is intended to be perceived." ;
  .

bf:contentAccessibility
  a owl:ObjectProperty ;
  rdfs:label "Content accessibility information" ;
  rdfs:comment "Suggested use - With Work or Instance" ;
  dcterms:modified
    "2016-04-21 (New)" ,
    "2017-02-03 (changed from data to object property)" ,
    "2017-03-15 (fixed typo in range)"
    ;
  rdfs:range bf:ContentAccessibility ;
  skos:definition "Information that assists those with a sensory impairment for greater understanding of content, e.g., captions." ;
  .

bf:continuedBy
  a owl:ObjectProperty ;
  rdfs:subPropertyOf bf:succeededBy ;
  rdfs:label "Continued by" ;
  rdfs:comment
    "Suggested use - With Work or Instance" ,
    "Suggested value - Work or Instance"
    ;
  dcterms:modified
    "2016-04-21 (New)" ,
    "2016-04-29 (added inverse, updated range)"
    ;
  owl:inverseOf bf:continues ;
  skos:definition "Resource whose content continues an earlier resource under a new title" ;
  .

bf:continuedInPartBy
  a owl:ObjectProperty ;
  rdfs:subPropertyOf bf:succeededBy ;
  rdfs:label "Continued in part by" ;
  rdfs:comment
    "Suggested use - With Work or Instance" ,
    "Suggested value - Work or Instance"
    ;
  dcterms:modified
    "2016-04-21 (New)" ,
    "2016-04-29 (added inverse, updated range)"
    ;
  owl:inverseOf bf:separatedFrom ;
  skos:definition "Resource part of whose content separated from an earlier resource to form a new resource" ;
  .

bf:continues
  a owl:ObjectProperty ;
  rdfs:subPropertyOf bf:precededBy ;
  rdfs:label "Continuation of" ;
  rdfs:comment
    "Suggested use - With Work or Instance" ,
    "Suggested value - Work or Instance"
    ;
  dcterms:modified
    "2016-04-21 (New)" ,
    "2016-04-29 (added inverse, updated range)"
    ;
  owl:inverseOf bf:continuedBy ;
  skos:definition "Resource that is continued by the content of a later resource under a new title" ;
  .

bf:continuesInPart
  a owl:ObjectProperty ;
  rdfs:subPropertyOf bf:precededBy ;
  rdfs:label "Continuation in part of" ;
  rdfs:comment
    "Suggested use - With Work or Instance" ,
    "Suggested value - Work or Instance"
    ;
  dcterms:modified
    "2016-04-21 (New)" ,
    "2016-04-29 (added inverse, updated range)"
    ;
  owl:inverseOf bf:splitInto ;
  skos:definition "Resource that split into two or more separate resources with new titles" ;
  .

bf:contribution
  a owl:ObjectProperty ;
  rdfs:label "Contributor and role" ;
  rdfs:comment "Suggested use - With Work, Instance or Item" ;
  dcterms:modified
    "2016-04-21 (New)" ,
    "2017-02-03 (Corrected label)"
    ;
  rdfs:range bf:Contribution ;
  skos:definition "Agent and its role in relation to the resource" ;
  .

bf:contributionOf
  a owl:ObjectProperty ;
  rdfs:label "Contribution of" ;
  rdfs:comment "Suggested value - Work, Instance or Item" ;
  dcterms:modified "2021-06-09 (New [GH4])" ;
  rdfs:domain bf:Contribution ;
  skos:definition "Relates a contribution resource, which associates an Agent and Role together, to the relevant resource" ;
  .

bf:coordinates
  a owl:DatatypeProperty ;
  rdfs:label "Cartographic coordinates" ;
  dcterms:modified "2016-04-21 (New)" ;
  rdfs:domain bf:Cartographic ;
  rdfs:range rdfs:Literal ;
  skos:definition "Mathematical system for identifying the area covered by the cartographic content of a resource, expressed either by means of longitude and latitude on the surface of planets or by the angles of right ascension and declination for celestial cartographic content." ;
  .

bf:copyrightDate
  a owl:DatatypeProperty ;
  rdfs:subPropertyOf bf:date ;
  rdfs:label "Copyright date" ;
  rdfs:comment "Suggested use - With Work or Instance" ;
  dcterms:modified "2016-04-21 (New)" ;
  rdfs:range rdfs:Literal ;
  skos:definition "Date associated with a claim of protection under copyright or a similar regime." ;
  .

bf:copyrightRegistration
  a owl:ObjectProperty ;
  rdfs:label "Copyright registration information" ;
  rdfs:comment "Suggested use - With Work or Instance" ;
  dcterms:modified
    "2016-04-21 (New)" ,
    "2016-05-04 (Corrected expected value)"
    ;
  rdfs:range bf:CopyrightRegistration ;
  skos:definition "Copyright and Legal Deposit registration information" ;
  .

bf:count
  a owl:DatatypeProperty ;
  rdfs:label "Number of units" ;
  dcterms:modified
    "2016-04-21 (New)" ,
    "2025-01-23 (Ontological correction - partially addresses [GH121])"
    ;
  rdfs:range rdfs:Literal ;
  skos:definition "Number associated with a measure of units, such as the number of units and/or subunits making up a resource." ;
  .

bf:coverArt
  a owl:ObjectProperty ;
  rdfs:label "Cover art" ;
  rdfs:comment "Suggested use - With Work or Instance" ;
  dcterms:modified "2016-04-21 (New)" ;
  rdfs:range bf:CoverArt ;
  skos:definition "Cover art image of a resource." ;
  .

bf:creationDate
  a owl:DatatypeProperty ;
  rdfs:subPropertyOf bf:date ;
  rdfs:label "Description creation date" ;
  dcterms:modified "2016-04-21 (New)" ;
  rdfs:domain bf:AdminMetadata ;
  rdfs:range rdfs:Literal ;
  skos:definition "Date or date and time on which the original metadata first created" ;
  .

bf:credits
  a owl:DatatypeProperty ;
  rdfs:label "Credits note" ;
  rdfs:comment "Suggested use - With Work or Instance" ;
  dcterms:modified "2016-04-21 (New)" ;
  rdfs:range rdfs:Literal ;
  skos:definition "Information in note form of credits for persons or organizations who have participated in the creation and/or production of the resource." ;
  .

bf:custodialHistory
  a owl:DatatypeProperty ;
  rdfs:label "Custodial history" ;
  rdfs:comment "Suggested use - With Work, Instance or Item" ;
  dcterms:modified
    "2016-04-21 (New)" ,
    "2021-06-09 (Added note [GH38])"
    ;
  rdfs:range rdfs:Literal ;
  skos:definition "Information about the provenance, such as origin, ownership and custodial history (chain of custody), of a resource." ;
  skos:editorialNote "See also the ARM Ontology for strategies to model this information in greater detail." ;
  .

bf:dataSource
  a owl:ObjectProperty ;
  rdfs:subPropertyOf bf:relatedTo ;
  rdfs:label "Data source" ;
  rdfs:comment
    "Suggested use - With Work or Instance" ,
    "Suggested value - Work or Instance"
    ;
  dcterms:modified
    "2016-04-21 (New)" ,
    "2016-04-29 (updated range)"
    ;
  skos:definition "Resource that is a data source to which the described resource is related; may contain information about other files, printed sources, or collection procedures" ;
  .

bf:date
  a owl:DatatypeProperty ;
  rdfs:label "Date" ;
  dcterms:modified
    "2016-04-21 (New)" ,
    "2025-01-23 (Removed defined range [GH125])"
    ;
  skos:definition "Date designation associated with a resource or element of description, such as date of title variation; year a degree was awarded; date associated with the publication, printing, distribution, issue, release or production of a resource. May be date typed." ;
  .

bf:degree
  a owl:DatatypeProperty ;
  rdfs:label "Degree" ;
  dcterms:modified "2016-04-21 (New)" ;
  rdfs:domain bf:Dissertation ;
  rdfs:range rdfs:Literal ;
  skos:definition "Degree for which author was a candidate." ;
  .

bf:derivativeOf
  a owl:ObjectProperty ;
  rdfs:subPropertyOf bf:relatedTo ;
  rdfs:label "Is derivative of" ;
  rdfs:comment
    "Suggested use - With Work or Instance" ,
    "Suggested value - Work or Instance"
    ;
  dcterms:modified
    "2016-04-21 (New)" ,
    "2016-04-29 (added inverse)"
    ;
  owl:inverseOf bf:hasDerivative ;
  skos:definition "Source work from which the described resource is derived" ;
  .

bf:derivedFrom
  a owl:ObjectProperty ;
  rdfs:label "Source metadata" ;
  dcterms:modified
    "2016-04-21 (New)" ,
    "2021-06-09 (Broadened range [GH41])" ,
    "2025-01-23 (Ontological correction - partially addresses [GH121])"
    ;
  rdfs:domain bf:AdminMetadata ;
  skos:definition "Link to the metadata that was the source of the data" ;
  .

bf:descriptionAuthentication
  a owl:ObjectProperty ;
  rdfs:label "Description authentication" ;
  dcterms:modified "2016-04-21 (New)" ;
  rdfs:domain bf:AdminMetadata ;
  rdfs:range bf:DescriptionAuthentication ;
  skos:definition "Indication of specific types of reviews that have been carried out on the description information" ;
  .

bf:descriptionConventions
  a owl:ObjectProperty ;
  rdfs:label "Description conventions" ;
  dcterms:modified
    "2016-04-21 (New)" ,
    "2016-04-24 (fixed domain name)"
    ;
  rdfs:domain bf:AdminMetadata ;
  rdfs:range bf:DescriptionConventions ;
  skos:definition "Rules used for the descriptive content of the resource description" ;
  .

bf:descriptionLanguage
  a owl:ObjectProperty ;
  rdfs:label "Description language" ;
  dcterms:modified "2016-04-21 (New)" ;
  rdfs:domain bf:AdminMetadata ;
  rdfs:range bf:Language ;
  skos:definition "Language used for the metadata" ;
  .

bf:descriptionLevel
  a owl:ObjectProperty ;
  rdfs:label "Description level" ;
  dcterms:modified "2022-10-03 (New [GH43])" ;
  rdfs:domain bf:AdminMetadata ;
  rdfs:range bf:DescriptionLevel ;
  skos:definition "Designation of the descriptive content of the metadata" ;
  .

bf:descriptionModifier
  a owl:ObjectProperty ;
  rdfs:label "Description modifier" ;
  dcterms:modified
    "2016-04-21 (New)" ,
    "2021-06-09 (Broadened range [GH63])" ,
    "2025-01-23 (Ontological correction - partially addresses [GH121])"
    ;
  rdfs:domain bf:AdminMetadata ;
  skos:definition "Agency that modified a description" ;
  .

bf:digitalCharacteristic
  a owl:ObjectProperty ;
  rdfs:label "Digital characteristic" ;
  dcterms:modified "2016-04-21 (New)" ;
  rdfs:domain bf:Instance ;
  rdfs:range bf:DigitalCharacteristic ;
  skos:definition "Technical specification relating to the digital encoding of text, image, audio, video, and other types of data in a resource." ;
  .

bf:dimensions
  a owl:DatatypeProperty ;
  rdfs:label "Dimensions" ;
  dcterms:modified
    "2016-04-21 (New)" ,
    "2021-06-09 (Added note [GH39])"
    ;
  rdfs:domain bf:Instance ;
  rdfs:range rdfs:Literal ;
  skos:definition "Measurements of the carrier or carriers and/or the container of a resource." ;
  skos:editorialNote "See also the ARM Ontology for strategies to model this information in greater detail." ;
  .

bf:dissertation
  a owl:ObjectProperty ;
  rdfs:label "Dissertation Information" ;
  rdfs:comment "Suggested use - With Work or Instance" ;
  dcterms:modified "2016-04-21 (New)" ;
  rdfs:range bf:Dissertation ;
  skos:definition "Work presented as part of the formal requirements for an academic degree." ;
  .

bf:distributionStatement
  a owl:DatatypeProperty ;
  rdfs:label "Distribution statement" ;
  dcterms:modified "2024-07-10 (New [GH124])" ;
  rdfs:domain bf:Instance ;
  rdfs:range rdfs:Literal ;
  skos:definition "Statement related to the distribution of the resources; usually transcribed." ;
  .

bf:duration
  a owl:DatatypeProperty ;
  rdfs:label "Duration" ;
  rdfs:comment "Suggested use - With Work or Instance" ;
  dcterms:modified "2016-04-21 (New)" ;
  rdfs:range rdfs:Literal ;
  skos:definition "Information about the playing time, running time, etc. of a resource." ;
  .

bf:edition
  a owl:DatatypeProperty ;
  rdfs:label "Classification scheme edition" ;
  dcterms:modified "2016-04-21 (New)" ;
  rdfs:domain bf:Classification ;
  rdfs:range rdfs:Literal ;
  skos:definition "Edition of the classification scheme, such as full, abridged or a number, when a classification scheme designates editions." ;
  .

bf:editionEnumeration
  a owl:DatatypeProperty ;
  rdfs:label "Edition enumeration" ;
  dcterms:modified "2016-04-21 (New)" ;
  rdfs:domain bf:Instance ;
  rdfs:range rdfs:Literal ;
  skos:definition "Enumeration of the edition; usually transcribed." ;
  .

bf:editionStatement
  a owl:DatatypeProperty ;
  rdfs:label "Edition statement" ;
  dcterms:modified "2016-04-21 (New)" ;
  rdfs:domain bf:Instance ;
  rdfs:range rdfs:Literal ;
  skos:definition "Information identifying the edition or version of the resource and associated statements of responsibility for the edition; usually transcribed." ;
  .

bf:electronicLocator
  a owl:ObjectProperty ;
  rdfs:label "Electronic location" ;
  dcterms:modified
    "2016-04-21 (New)" ,
    "2021-06-09 (Removed domain [GH66])" ,
    "2025-01-23 (Ontological correction - partially addresses [GH121])"
    ;
  skos:definition "Electronic location from which the resource is available." ;
  .

bf:emulsion
  a owl:ObjectProperty ;
  rdfs:label "Emulsion" ;
  dcterms:modified "2016-04-21 (New)" ;
  rdfs:domain bf:Instance ;
  rdfs:range bf:Emulsion ;
  skos:definition "Suspension of light-sensitive chemicals used as a coating on a microfilm or microfiche, e.g., silver halide." ;
  .

bf:ensemble
  a owl:ObjectProperty ;
  rdfs:label "Ensemble" ;
  dcterms:modified
    "2016-04-21 (New)" ,
    "2021-06-09 (Changed domain [GH56], Modified definition [GH56])"
    ;
  rdfs:domain bf:Work ;
  rdfs:range bf:Ensemble ;
  skos:definition "Ensemble applicable to the Work." ;
  .

bf:ensembleType
  a owl:DatatypeProperty ;
  rdfs:label "Ensemble type" ;
  dcterms:modified
    "2016-04-21 (New)" ,
    "2021-06-09 (Changed domain [GH56])"
    ;
  rdfs:domain bf:Ensemble ;
  rdfs:range rdfs:Literal ;
  skos:definition "Specific type of ensemble, such as orchestra, band, guitar ensemble." ;
  .

bf:enumerationAndChronology
  a owl:ObjectProperty ;
  rdfs:label "Numbering or other enumeration and dates associated with issues or items held." ;
  dcterms:modified "2016-04-21 (New)" ;
  rdfs:domain bf:Item ;
  rdfs:range bf:EnumerationAndChronology ;
  skos:definition "Numbering and dates of issues or items held." ;
  .

bf:equinox
  a owl:DatatypeProperty ;
  rdfs:label "Cartographic equinox" ;
  dcterms:modified "2016-04-21 (New)" ;
  rdfs:domain bf:Cartographic ;
  rdfs:range rdfs:Literal ;
  skos:definition "One of two points of intersection of the ecliptic and the celestial equator, occupied by the sun when its declination is 0 degrees." ;
  .

bf:eventContent
  a owl:ObjectProperty ;
  rdfs:subPropertyOf bf:relatedTo ;
  rdfs:label "Event content" ;
  dcterms:modified
    "2016-04-21 (New)" ,
    "2016-04-29 (added inverse)"
    ;
  rdfs:domain bf:Event ;
  rdfs:range bf:Work ;
  owl:inverseOf bf:eventContentOf ;
  skos:definition "Work whose content is the described event" ;
  .

bf:eventContentOf
  a owl:ObjectProperty ;
  rdfs:subPropertyOf bf:relatedTo ;
  rdfs:label "Has event content" ;
  dcterms:modified
    "2016-04-21 (New)" ,
    "2016-04-29 (added inverse)"
    ;
  rdfs:domain bf:Work ;
  rdfs:range bf:Event ;
  owl:inverseOf bf:eventContent ;
  skos:definition "Event that is the content of the described work" ;
  .

bf:exclusionGRing
  a owl:DatatypeProperty ;
  rdfs:label "Cartographic G ring area excluded" ;
  dcterms:modified "2016-04-21 (New)" ;
  rdfs:domain bf:Cartographic ;
  rdfs:range rdfs:Literal ;
  skos:definition "Coordinate pairs that identify the closed non-intersecting boundary of the area contained within the G-polygon outer ring that is excluded." ;
  .

bf:expressionOf
  a owl:ObjectProperty ;
  rdfs:subPropertyOf bf:relatedTo ;
  rdfs:label "Expression of" ;
  rdfs:comment
    "Suggested use - With Work or Hub" ,
    "Suggested value - With Work or Hub"
    ;
  dcterms:modified
    "2016-04-21 (New)" ,
    "2016-04-29 (added inverse)" ,
    "2021-06-09 (Modified definition [GH8])" ,
    "2023-11-30 (Modified domain/range to support Hub [GH110])"
    ;
  owl:inverseOf bf:hasExpression ;
  skos:definition "Work or Hub that the described Work or Hub is an expression of; used to connect Works and/or Hubs under LRM/RDA guidelines or similar implementations" ;
  .

bf:extent
  a owl:ObjectProperty ;
  rdfs:label "Extent" ;
  dcterms:modified
    "2016-04-21 (New)" ,
    "2021-06-09 (Broadened range [GH30])" ,
    "2025-01-23 (Ontological correction - partially addresses [GH121])"
    ;
  rdfs:range bf:Extent ;
  skos:definition "Number and type of units and/or subunits making up a resource." ;
  .

bf:findingAid
  a owl:ObjectProperty ;
  rdfs:subPropertyOf bf:accompaniedBy ;
  rdfs:label "Finding aid" ;
  rdfs:comment
    "Suggested use - With Work or Instance" ,
    "Suggested value - Work or Instance"
    ;
  dcterms:modified
    "2016-04-21 (New)" ,
    "2016-04-29 (added inverse, updated range)"
    ;
  owl:inverseOf bf:findingAidOf ;
  skos:definition "Relationship for archival, visual, and manuscript resources to a finding aid or similar control materials" ;
  .

bf:findingAidOf
  a owl:ObjectProperty ;
  rdfs:subPropertyOf bf:accompanies ;
  rdfs:label "Finding aid for" ;
  rdfs:comment
    "Suggested use - With Work or Instance" ,
    "Suggested value - Work or Instance"
    ;
  dcterms:modified
    "2016-04-21 (New)" ,
    "2016-04-29 (added inverse, updated range)"
    ;
  owl:inverseOf bf:findingAid ;
  skos:definition "Finding aid or similar control materials for archival, visual, and manuscript resources" ;
  .

bf:firstIssue
  a owl:DatatypeProperty ;
  rdfs:label "Multipart first issue" ;
  dcterms:modified
    "2016-04-21 (New)" ,
    "2021-06-09 (Removed domain [GH76])" ,
    "2025-01-23 (Ontological correction - partially addresses [GH121])"
    ;
  rdfs:range rdfs:Literal ;
  skos:definition "Beginning date of a resource and/or the sequential designations." ;
  .

bf:fontSize
  a owl:ObjectProperty ;
  rdfs:label "Font size" ;
  dcterms:modified
    "2016-04-21 (New)" ,
    "2021-06-09 (Added note [GH40])"
    ;
  rdfs:domain bf:Instance ;
  rdfs:range bf:FontSize ;
  skos:definition "Size of the type used to represent the characters and symbols in a resource." ;
  skos:editorialNote "See also the ARM Ontology for strategies to model this information in greater detail." ;
  .

bf:frequency
  a owl:ObjectProperty ;
  rdfs:label "Frequency" ;
  dcterms:modified
    "2016-04-21 (New)" ,
    "2021-06-09 (Removed domain [GH76])" ,
    "2025-01-23 (Ontological correction - partially addresses [GH121])"
    ;
  rdfs:range bf:Frequency ;
  skos:definition "Intervals at which the parts of a serially produced resource or the updates to an integrating resource are issued." ;
  .

bf:generation
  a owl:ObjectProperty ;
  rdfs:label "Generation" ;
  dcterms:modified "2016-04-21 (New)" ;
  rdfs:domain bf:Instance ;
  rdfs:range bf:Generation ;
  skos:definition "Relationship between an original carrier and the carrier of a reproduction made from the original." ;
  .

bf:generationDate
  a owl:DatatypeProperty ;
  rdfs:subPropertyOf bf:date ;
  rdfs:label "Date generated" ;
  dcterms:modified "2016-04-21 (New)" ;
  rdfs:domain bf:AdminMetadata ;
  rdfs:range rdfs:Literal ;
  skos:definition "Date of conversion of the metadata from another format" ;
  .

bf:generationProcess
  a owl:ObjectProperty ;
  rdfs:label "Description generation" ;
  dcterms:modified "2016-04-21 (New)" ;
  rdfs:domain bf:AdminMetadata ;
  rdfs:range bf:GenerationProcess ;
  skos:definition "Indication of the program or process used to generate the description by application of a particular transformation" ;
  .

bf:genreForm
  a owl:ObjectProperty ;
  rdfs:label "Genre/form" ;
  rdfs:comment
    "Suggested use - With Work, Instance or Item" ,
    "Suggested value - bf:GenreForm or madsrdf:GenreForm or skos:Concept"
    ;
  dcterms:modified
    "2016-04-21 (New)" ,
    "2021-06-09 (Broadened range [GH16])" ,
    "2025-01-23 (Ontological correction - partially addresses [GH121])"
    ;
  skos:definition "Form category or genre to which a resource belongs" ;
  .

bf:geographicCoverage
  a owl:ObjectProperty ;
  rdfs:label "Geographic coverage" ;
  rdfs:comment "Suggested value - bf:GeographicCoverage or bf:Place or madsrdf:Geographic" ;
  dcterms:modified
    "2016-04-21 (New)" ,
    "2017-02-06 (Changed from data to object property)" ,
    "2021-06-09 (Removed domain [GH15])" ,
    "2025-01-23 (Ontological correction - partially addresses [GH121])"
    ;
  skos:definition "Geographic coverage of the content of the resource." ;
  .

bf:grantingInstitution
  a owl:ObjectProperty ;
  rdfs:label "Degree issuing institution" ;
  dcterms:modified
    "2016-04-21 (New)" ,
    "2021-06-09 (Broadened range [GH63])" ,
    "2025-01-23 (Ontological correction - partially addresses [GH121])"
    ;
  rdfs:domain bf:Dissertation ;
  skos:definition "Name of degree granting institution." ;
  .

bf:hasDerivative
  a owl:ObjectProperty ;
  rdfs:subPropertyOf bf:relatedTo ;
  rdfs:label "Has derivative" ;
  rdfs:comment
    "Suggested use - With Work or Instance" ,
    "Suggested value - Work or Instance"
    ;
  dcterms:modified
    "2016-04-21 (New)" ,
    "2016-04-29 (added inverse)"
    ;
  owl:inverseOf bf:derivativeOf ;
  skos:definition "Resource that is a modification of the described work" ;
  .

bf:hasEquivalent
  a owl:SymmetricProperty ;
  rdfs:subPropertyOf bf:relatedTo ;
  rdfs:label "Equivalence" ;
  rdfs:comment
    "Suggested use - With Work, Instance or Item" ,
    "Suggested value - Work, Instance or Item"
    ;
  dcterms:modified "2016-04-21 (New)" ;
  skos:definition "Resource embodies the same content as the described resource" ;
  .

bf:hasExpression
  a owl:ObjectProperty ;
  rdfs:subPropertyOf bf:relatedTo ;
  rdfs:label "Expressed as" ;
  rdfs:comment
    "Suggested use - With Work or Hub" ,
    "Suggested value - With Work or Hub"
    ;
  dcterms:modified
    "2016-04-21 (New)" ,
    "2016-04-29 (added inverse)" ,
    "2021-06-09 (Modified definition [GH8])" ,
    "2023-11-30 (Modified domain/range to support Hub [GH110])"
    ;
  owl:inverseOf bf:expressionOf ;
  skos:definition "Work or Hub that is an expression of a described Work or Hub; used to relate Works and/or Hubs under LRM/RDA guidelines or similar implementations" ;
  .

bf:hasInstance
  a owl:ObjectProperty ;
  rdfs:subPropertyOf bf:relatedTo ;
  rdfs:label "Instance of Work" ;
  dcterms:modified
    "2016-04-21 (New)" ,
    "2016-04-29 (added inverse)"
    ;
  rdfs:domain bf:Work ;
  rdfs:range bf:Instance ;
  owl:inverseOf bf:instanceOf ;
  skos:definition "Instance is related to described Work ; used to connect Works to Instances in the BIBFRAME structure" ;
  .

bf:hasItem
  a owl:ObjectProperty ;
  rdfs:subPropertyOf bf:relatedTo ;
  rdfs:label "Has holding" ;
  dcterms:modified
    "2016-04-21 (New)" ,
    "2016-04-29 (added inverse)" ,
    "2017-02-07 (slight revision of definition)"
    ;
  rdfs:domain bf:Instance ;
  rdfs:range bf:Item ;
  owl:inverseOf bf:itemOf ;
  skos:definition "Item which is an example of the described Instance" ;
  .

bf:hasPart
  a owl:ObjectProperty ;
  rdfs:subPropertyOf bf:relatedTo ;
  rdfs:label "Has part" ;
  rdfs:comment
    "Suggested use - With Work, Instance, Item or Event" ,
    "Suggested value - Work, Instance, Item or Event"
    ;
  dcterms:modified
    "2016-04-21 (New)" ,
    "2016-04-29 (added inverse)" ,
    "2021-06-09 (Use with Event also [GH9])"
    ;
  owl:inverseOf bf:partOf ;
  skos:definition "Resource that is included either physically or logically in the described resource" ;
  .

bf:hasReproduction
  a owl:ObjectProperty ;
  rdfs:subPropertyOf bf:hasEquivalent ;
  rdfs:label "Reproduced as" ;
  dcterms:modified
    "2016-04-21 (New)" ,
    "2016-04-29 (added inverse)"
    ;
  rdfs:domain bf:Instance ;
  rdfs:range bf:Instance ;
  owl:inverseOf bf:reproductionOf ;
  skos:definition "Resource that reproduces another Resource" ;
  .

bf:hasSeries
  a owl:ObjectProperty ;
  rdfs:subPropertyOf bf:partOf ;
  rdfs:label "In series" ;
  rdfs:comment
    "Suggested use - With Work or Instance" ,
    "Suggested value - Work or Instance"
    ;
  dcterms:modified
    "2016-04-21 (New)" ,
    "2016-04-29 (added inverse, updated range)" ,
    "2024-07-10 (updated definition [GF106])"
    ;
  owl:inverseOf bf:seriesOf ;
  skos:definition "Relation between a resource and the larger resource in which it has been issued; the title of the encompassing larger resource features on the part" ;
  .

bf:hasSubseries
  a owl:ObjectProperty ;
  rdfs:subPropertyOf bf:partOf ;
  rdfs:label "Subseries" ;
  rdfs:comment
    "Suggested use - With Work or Instance" ,
    "Suggested value - Work or Instance"
    ;
  dcterms:modified
    "2016-04-21 (New)" ,
    "2016-04-29 (added inverse, updated range)" ,
    "2024-07-10 (updated definition [GF106])"
    ;
  owl:inverseOf bf:subseriesOf ;
  skos:definition "Relation between a resource and the larger Series resource in which it has been issued; the larger Series resource is part of another overarching Series resource" ;
  .

bf:heldBy
  a owl:ObjectProperty ;
  rdfs:label "Held by" ;
  dcterms:modified
    "2016-04-21 (New)" ,
    "2021-06-09 (Broadened range [GH63])" ,
    "2025-01-23 (Ontological correction - partially addresses [GH121])"
    ;
  rdfs:domain bf:Item ;
  skos:definition "Entity holding the item or from which it is available." ;
  .

bf:hierarchicalLevel
  a owl:DatatypeProperty ;
  rdfs:label "Hierarchical level of material" ;
  dcterms:modified
    "2016-04-21 (New)" ,
    "2021-06-09 (Modified range [GH77])"
    ;
  rdfs:domain bf:CollectionArrangement ;
  rdfs:range rdfs:Literal ;
  skos:definition "Hierarchical position of the described materials relative to other material from the same source." ;
  .

bf:historyOfWork
  a owl:DatatypeProperty ;
  rdfs:label "History of the work" ;
  dcterms:modified "2016-04-21 (New)" ;
  rdfs:domain bf:Work ;
  rdfs:range rdfs:Literal ;
  skos:definition "Information about the history of a Work." ;
  .

bf:identifiedBy
  a owl:ObjectProperty ;
  rdfs:label "Identifier" ;
  dcterms:modified
    "2016-04-21 (New)" ,
    "2017-05-04 (New inverse)" ,
    "2025-01-23 (Ontological correction - partially addresses [GH121])"
    ;
  rdfs:range bf:Identifier ;
  owl:inverseOf bf:identifies ;
  skos:definition "Character string associated with a resource that serves to differentiate that resource from other resources, i.e., that uniquely identifies an entity." ;
  .

bf:identifies
  a owl:ObjectProperty ;
  rdfs:label "Resource identified" ;
  dcterms:modified
    "2017-02-03 (New inverse)" ,
    "2025-01-23 (Ontological correction - partially addresses [GH121])"
    ;
  rdfs:domain bf:Identifier ;
  owl:inverseOf bf:identifiedBy ;
  skos:definition "Resource that is associated with a character string that serves to differentiate one resource from another." ;
  .

bf:illustrativeContent
  a owl:ObjectProperty ;
  rdfs:label "Illustrative content information" ;
  rdfs:comment "Suggested use - With Work or Instance" ;
  dcterms:modified "2016-04-21 (New)" ;
  rdfs:range bf:Illustration ;
  skos:definition "Information about content intended to illustrate a resource." ;
  .

bf:immediateAcquisition
  a owl:ObjectProperty ;
  rdfs:label "Immediate acquisition" ;
  dcterms:modified
    "2016-04-21 (New)" ,
    "2017-02-06 (Changed from data to object property)"
    ;
  rdfs:domain bf:Item ;
  rdfs:range bf:ImmediateAcquisition ;
  skos:definition "Information about the circumstances, e.g., source, date, method, under which the resource was directly acquired." ;
  .

bf:index
  a owl:ObjectProperty ;
  rdfs:subPropertyOf bf:accompaniedBy ;
  rdfs:label "Has index" ;
  rdfs:comment
    "Suggested use - With Work or Instance" ,
    "Suggested value - Work or Instance"
    ;
  dcterms:modified
    "2016-04-21 (New)" ,
    "2016-04-29 (added inverse, updated range)" ,
    "2017-02-03 (corrected label)"
    ;
  owl:inverseOf bf:indexOf ;
  skos:definition "Resource has an accompanying index" ;
  .

bf:indexOf
  a owl:ObjectProperty ;
  rdfs:subPropertyOf bf:accompanies ;
  rdfs:label "Index to" ;
  rdfs:comment
    "Suggested use - With Work or Instance" ,
    "Suggested value - Work or Instance"
    ;
  dcterms:modified
    "2016-04-21 (New)" ,
    "2016-04-29 (added inverse, updated range)"
    ;
  owl:inverseOf bf:index ;
  skos:definition "Index that accompanies a resource" ;
  .

bf:instanceOf
  a owl:ObjectProperty ;
  rdfs:subPropertyOf bf:relatedTo ;
  rdfs:label "Instance of" ;
  dcterms:modified
    "2016-04-21 (New)" ,
    "2016-04-29 (added inverse)"
    ;
  rdfs:domain bf:Instance ;
  rdfs:range bf:Work ;
  owl:inverseOf bf:hasInstance ;
  skos:definition "Work the Instance described instantiates or manifests; used to connect Instances to Works in the BIBFRAME structure" ;
  .

bf:instrument
  a owl:ObjectProperty ;
  rdfs:label "Instrument" ;
  dcterms:modified "2016-04-21 (New)" ;
  rdfs:domain bf:Work ;
  rdfs:range bf:MusicInstrument ;
  skos:definition "Instrument for which a musical Work is appropriate." ;
  .

bf:instrumentalType
  a owl:DatatypeProperty ;
  rdfs:label "Instrument role" ;
  dcterms:modified "2016-04-21 (New)" ;
  rdfs:domain bf:MusicInstrument ;
  rdfs:range rdfs:Literal ;
  skos:definition "Specific role of instrument, such as alternate, doubling, solo, ensemble." ;
  .

bf:intendedAudience
  a owl:ObjectProperty ;
  rdfs:label "Intended audience" ;
  rdfs:comment "Suggested use - With Work or Instance" ;
  dcterms:modified
    "2016-04-21 (New)" ,
    "2022-10-03 (Broadened range [GH74])" ,
    "2025-01-23 (Ontological correction - partially addresses [GH121])"
    ;
  skos:definition "Information that identifies the specific audience or intellectual level for which the content of the resource is considered appropriate." ;
  .

bf:issuance
  a owl:ObjectProperty ;
  rdfs:label "Mode of issuance" ;
  rdfs:comment "Suggested use - With Work or Instance" ;
  dcterms:modified "2016-04-21 (New)" ;
  rdfs:range bf:Issuance ;
  skos:definition "Categorization reflecting whether a resource is issued in one or more parts, the way it is updated, and its intended termination." ;
  .

bf:issuedWith
  a owl:SymmetricProperty ;
  rdfs:subPropertyOf bf:accompanies ;
  rdfs:label "Issued with" ;
  rdfs:comment
    "Suggested use - With Work or Instance" ,
    "Suggested value - Work or Instance"
    ;
  dcterms:modified
    "2016-04-21 (New)" ,
    "2021-06-09 (Broadened range [GH62], Broadened domain [GH62])"
    ;
  skos:definition "Resource that is issued on the same carrier as the resource being described" ;
  .

bf:itemOf
  a owl:ObjectProperty ;
  rdfs:subPropertyOf bf:relatedTo ;
  rdfs:label "Holding for" ;
  dcterms:modified
    "2016-04-21 (New)" ,
    "2016-04-29 (added inverse)" ,
    "2017-02-07 (slight revision of definition)"
    ;
  rdfs:domain bf:Item ;
  rdfs:range bf:Instance ;
  owl:inverseOf bf:hasItem ;
  skos:definition "Instance for which the described Item is an example" ;
  .

bf:itemPortion
  a owl:DatatypeProperty ;
  rdfs:label "Classification item number" ;
  dcterms:modified "2016-04-21 (New)" ;
  rdfs:domain bf:Classification ;
  rdfs:range rdfs:Literal ;
  skos:definition "Number attached to a classification string that indicates a particular item." ;
  .

bf:language
  a owl:ObjectProperty ;
  rdfs:label "Language information" ;
  rdfs:comment "Suggested value - bf:Language or madsrdf:Language" ;
  dcterms:modified
    "2016-04-21 (New)" ,
    "2022-10-03 (Broadened range [GH70])" ,
    "2025-01-23 (Ontological correction - partially addresses [GH121])"
    ;
  skos:definition "Language associated with a resource or its parts." ;
  .

bf:lastIssue
  a owl:DatatypeProperty ;
  rdfs:label "Multipart last issue" ;
  dcterms:modified
    "2016-04-21 (New)" ,
    "2021-06-09 (Removed domain [GH76])" ,
    "2025-01-23 (Ontological correction - partially addresses [GH121])"
    ;
  rdfs:range rdfs:Literal ;
  skos:definition "Ending date of a resource and/or the sequential designations." ;
  .

bf:layout
  a owl:ObjectProperty ;
  rdfs:label "Layout" ;
  dcterms:modified "2016-04-21 (New)" ;
  rdfs:domain bf:Instance ;
  rdfs:range bf:Layout ;
  skos:definition "Arrangement of text, images, tactile notation, etc., in a resource." ;
  .

bf:legalDate
  a owl:DatatypeProperty ;
  rdfs:subPropertyOf bf:date ;
  rdfs:label "Date of legal work" ;
  dcterms:modified "2016-04-21 (New)" ;
  rdfs:domain bf:Work ;
  rdfs:range rdfs:Literal ;
  skos:definition "Date of legal work, or promulgation of a law, or signing of a treaty." ;
  .

bf:mainTitle
  a owl:DatatypeProperty ;
  rdfs:label "Main title" ;
  dcterms:modified "2016-04-21 (New)" ;
  rdfs:domain bf:Title ;
  rdfs:range rdfs:Literal ;
  skos:definition "Title being addressed. Possible title component." ;
  .

bf:manufactureStatement
  a owl:DatatypeProperty ;
  rdfs:label "Manufacture statement" ;
  dcterms:modified "2024-07-10 (New [GH124])" ;
  rdfs:domain bf:Instance ;
  rdfs:range rdfs:Literal ;
  skos:definition "Statement related to the manufacture of the resources; usually transcribed." ;
  .

bf:material
  a owl:ObjectProperty ;
  rdfs:label "Material" ;
  rdfs:comment "Suggested use - With Work, Instance or Item" ;
  dcterms:modified
    "2021-06-09 (New [GH26])" ,
    "2025-01-23 (Ontological correction - partially addresses [GH121])"
    ;
  skos:definition "Resource uses, is composed of, integrates, etc. the related material." ;
  .

bf:materialOf
  a owl:ObjectProperty ;
  rdfs:label "Material of" ;
  rdfs:comment "Suggested use - With Work, Instance or Item" ;
  dcterms:modified
    "2021-06-09 (New [GH26])" ,
    "2025-01-23 (Ontological correction - partially addresses [GH121])"
    ;
  skos:definition "This material is related to a resource." ;
  .

bf:media
  a owl:ObjectProperty ;
  rdfs:label "Media type" ;
  rdfs:comment
    "Suggested use - With Work or Instance" ,
    "Suggested value - bf:Media or skos:Concept"
    ;
  dcterms:modified
    "2016-04-21 (New)" ,
    "2022-10-03 (Broadened range [GH73])" ,
    "2025-01-23 (Ontological correction - partially addresses [GH121])"
    ;
  skos:definition "Categorization reflecting the general type of intermediation device required to view, play, run, etc., the content of a resource." ;
  .

bf:mergedToForm
  a owl:ObjectProperty ;
  rdfs:subPropertyOf bf:succeededBy ;
  rdfs:label "Merged to form" ;
  rdfs:comment
    "Suggested use - With Work or Instance" ,
    "Suggested value - Work or Instance"
    ;
  dcterms:modified
    "2016-04-21 (New)" ,
    "2016-04-29 (added inverse, updated range)"
    ;
  owl:inverseOf bf:mergerOf ;
  skos:definition "One of two or more resources that come together to form a new resource" ;
  .

bf:mergerOf
  a owl:ObjectProperty ;
  rdfs:subPropertyOf bf:precededBy ;
  rdfs:label "Merger of" ;
  rdfs:comment
    "Suggested use - With Work or Instance" ,
    "Suggested value - Work or Instance"
    ;
  dcterms:modified
    "2016-04-21 (New)" ,
    "2016-04-29 (added inverse, updated range)"
    ;
  owl:inverseOf bf:mergedToForm ;
  skos:definition "One of two or more resources which came together to form a new resource" ;
  .

bf:mount
  a owl:ObjectProperty ;
  rdfs:label "Mount material or object" ;
  dcterms:modified
    "2016-04-21 (New)" ,
    "2021-06-09 (Modified label [GH29])" ,
    "2025-01-23 (Ontological correction - partially addresses [GH121])"
    ;
  rdfs:domain bf:Instance ;
  skos:definition "Physical material or object used for the support or backing to which the base material of a resource has been attached." ;
  .

bf:musicFormat
  a owl:ObjectProperty ;
  rdfs:label "Format of notated music" ;
  rdfs:comment "Suggested use - With Work or Instance" ;
  dcterms:modified "2016-04-21 (New)" ;
  rdfs:range bf:MusicFormat ;
  skos:definition "Layout for content of a resource that is presented in the form of musical notation, such as full score, condensed score, vocal score, etc." ;
  .

bf:musicKey
  a owl:DatatypeProperty ;
  rdfs:label "Music key" ;
  dcterms:modified "2016-04-21 (New)" ;
  rdfs:domain bf:Work ;
  rdfs:range rdfs:Literal ;
  skos:definition "Pitch and mode for music." ;
  .

bf:musicMedium
  a owl:ObjectProperty ;
  rdfs:label "Music medium of performance" ;
  dcterms:modified "2016-04-21 (New)" ;
  rdfs:domain bf:Work ;
  rdfs:range bf:MusicMedium ;
  skos:definition "Instrumental, vocal, and/or other medium of performance for which a musical resource was originally conceived, written or performed." ;
  .

bf:musicOpusNumber
  a owl:DatatypeProperty ;
  rdfs:label "Music opus number" ;
  dcterms:modified "2016-04-21 (New)" ;
  rdfs:domain bf:Work ;
  rdfs:range rdfs:Literal ;
  skos:definition "Numeric designation of a musical work assigned by a composer, publisher, or a musicologist." ;
  .

bf:musicSerialNumber
  a owl:DatatypeProperty ;
  rdfs:label "Music serial number" ;
  dcterms:modified "2016-04-21 (New)" ;
  rdfs:domain bf:Work ;
  rdfs:range rdfs:Literal ;
  skos:definition "Numeric designation for musical works consecutively numbered in music reference sources." ;
  .

bf:musicThematicNumber
  a owl:DatatypeProperty ;
  rdfs:label "Music thematic number" ;
  dcterms:modified "2016-04-21 (New)" ;
  rdfs:domain bf:Work ;
  rdfs:range rdfs:Literal ;
  skos:definition "Numeric designation for a musical work as found in a thematic index for the composer." ;
  .

bf:natureOfContent
  a owl:DatatypeProperty ;
  rdfs:label "Content nature" ;
  rdfs:comment "Suggested use - With Work or Instance" ;
  dcterms:modified "2016-04-21 (New)" ;
  rdfs:range rdfs:Literal ;
  skos:definition "Characterization that epitomizes the primary content of a resource, e.g., field recording of birdsong; combined time series analysis and graph plotting system." ;
  .

bf:notation
  a owl:ObjectProperty ;
  rdfs:label "Notation system" ;
  rdfs:comment "Suggested use - With Work or Instance" ;
  dcterms:modified "2016-04-21 (New)" ;
  rdfs:range bf:Notation ;
  skos:definition "Alphabet, script, or symbol system used to convey the content of the resource, including specialized scripts, typefaces, tactile notation, movement notation, and musical notation." ;
  .

bf:note
  a owl:ObjectProperty ;
  rdfs:label "Note" ;
  dcterms:modified
    "2016-04-21 (New)" ,
    "2025-01-23 (Ontological correction - partially addresses [GH121])"
    ;
  rdfs:range bf:Note ;
  skos:definition "General textual information relating to a resource, such as Information about a specific copy of a resource or information about a particular attribute of a resource." ;
  .

bf:noteFor
  a owl:ObjectProperty ;
  rdfs:label "Note for" ;
  dcterms:modified
    "2021-06-09 (New [GH34])" ,
    "2025-01-23 (Ontological correction - partially addresses [GH121])"
    ;
  rdfs:domain bf:Note ;
  skos:definition "Relates a Note resource to the resource to which the note pertains." ;
  .

bf:noteType
  a owl:DatatypeProperty ;
  rdfs:label "Note type" ;
  dcterms:modified "2016-04-21 (New)" ;
  rdfs:domain bf:Note ;
  rdfs:range rdfs:Literal ;
  skos:definition "Type of note." ;
  .

bf:originDate
  a owl:DatatypeProperty ;
  rdfs:subPropertyOf bf:date ;
  rdfs:label "Origin date" ;
  dcterms:modified
    "2016-04-21 (New)" ,
    "2021-06-09 (Better align definition with property name [GH50])" ,
    "2025-01-23 (Ontological correction - partially addresses [GH121])"
    ;
  rdfs:domain bf:Work ;
  skos:definition "Date or date range associated with the creation of a Work." ;
  .

bf:originPlace
  a owl:ObjectProperty ;
  rdfs:subPropertyOf bf:place ;
  rdfs:label "Origin place" ;
  rdfs:comment
    "Suggested use - With Work or Instance" ,
    "Suggested value - bf:Place or madsrdf:Geographic"
    ;
  dcterms:modified
    "2016-04-21 (New)" ,
    "2021-06-09 (Better align definition with property name [GH50], Broadened range [GH19])" ,
    "2022-10-03 (updated domain [GH83])" ,
    "2025-01-23 (Ontological correction - partially addresses [GH121])"
    ;
  skos:definition "Place from which the creation of the resource originated." ;
  .

bf:originalVersion
  a owl:ObjectProperty ;
  rdfs:subPropertyOf bf:derivativeOf ;
  rdfs:label "Original version" ;
  rdfs:comment
    "Suggested use - With Work or Instance" ,
    "Suggested value - Work or Instance"
    ;
  dcterms:modified
    "2016-04-21 (New)" ,
    "2016-04-29 (added inverse, updated range)"
    ;
  owl:inverseOf bf:originalVersionOf ;
  skos:definition "Resource is the original version of which this resource is a reproduction" ;
  .

bf:originalVersionOf
  a owl:ObjectProperty ;
  rdfs:subPropertyOf bf:hasDerivative ;
  rdfs:label "Original version of" ;
  rdfs:comment
    "Suggested use - With Work or Instance" ,
    "Suggested value - Work or Instance"
    ;
  dcterms:modified
    "2016-04-21 (New)" ,
    "2016-04-29 (added inverse, updated range)"
    ;
  owl:inverseOf bf:originalVersion ;
  skos:definition "Original version of a resource" ;
  .

bf:otherEdition
  a owl:SymmetricProperty ;
  rdfs:subPropertyOf bf:relatedTo ;
  rdfs:label "Other edition" ;
  rdfs:comment
    "Suggested use - With Work or Instance" ,
    "Suggested value - Work or Instance"
    ;
  dcterms:modified
    "2016-04-21 (New)" ,
    "2016-05-13 (symmetrical)" ,
    "2021-06-09 (Change subproperty to relatedTo [GH61])"
    ;
  skos:definition "Resource has other available editions, for example simultaneously published language editions or reprints" ;
  .

bf:otherPhysicalFormat
  a owl:SymmetricProperty ;
  rdfs:subPropertyOf bf:hasEquivalent ;
  rdfs:label "Has other physical format" ;
  rdfs:comment "Suggested use - With Work or Instance" ;
  dcterms:modified
    "2016-04-21 (New)" ,
    "2021-06-09 (Broadened domain [GH79])"
    ;
  rdfs:range bf:Instance ;
  skos:definition "Resource that is manifested in another physical carrier" ;
  .

bf:outerGRing
  a owl:DatatypeProperty ;
  rdfs:label "Cartographic outer G ring area covered" ;
  dcterms:modified "2016-04-21 (New)" ;
  rdfs:domain bf:Cartographic ;
  rdfs:range rdfs:Literal ;
  skos:definition "Coordinate pairs that identify the closed non-intersecting boundary of the area covered." ;
  .

bf:part
  a owl:DatatypeProperty ;
  rdfs:label "Part" ;
  dcterms:modified
    "2016-04-21 (New)" ,
    "2025-01-23 (Ontological correction - partially addresses [GH121])"
    ;
  rdfs:range rdfs:Literal ;
  skos:definition "Part of a resource to which information applies." ;
  .

bf:partName
  a owl:DatatypeProperty ;
  rdfs:label "Part title" ;
  dcterms:modified "2016-04-21 (New)" ;
  rdfs:domain bf:Title ;
  rdfs:range rdfs:Literal ;
  skos:definition "Part or section name of a title. Possible title component." ;
  .

bf:partNumber
  a owl:DatatypeProperty ;
  rdfs:label "Part number" ;
  dcterms:modified "2016-04-21 (New)" ;
  rdfs:domain bf:Title ;
  rdfs:range rdfs:Literal ;
  skos:definition "Part or section enumeration of a title. Possible title component." ;
  .

bf:partOf
  a owl:ObjectProperty ;
  rdfs:subPropertyOf bf:relatedTo ;
  rdfs:label "Is part of" ;
  rdfs:comment
    "Suggested use - With Work, Instance, Item or Event" ,
    "Suggested value - Work, Instance, Item or Event"
    ;
  dcterms:modified
    "2016-04-21 (New)" ,
    "2016-04-29 (added inverse)" ,
    "2021-06-09 (Use with Event also [GH9])"
    ;
  owl:inverseOf bf:hasPart ;
  skos:definition "Resource in which the described resource is physically or logically contained" ;
  .

bf:pattern
  a owl:DatatypeProperty ;
  rdfs:label "Arrangement of material" ;
  dcterms:modified
    "2016-04-21 (New)" ,
    "2021-06-09 (Modified range [GH77])"
    ;
  rdfs:domain bf:CollectionArrangement ;
  rdfs:range rdfs:Literal ;
  skos:definition "Pattern of arrangement of materials within a unit." ;
  .

bf:physicalLocation
  a owl:DatatypeProperty ;
  rdfs:label "Storing or shelving location" ;
  dcterms:modified "2016-04-21 (New)" ;
  rdfs:domain bf:Item ;
  rdfs:range rdfs:Literal ;
  skos:definition "Location in the holding agency where the item is shelved or stored." ;
  .

bf:place
  a owl:ObjectProperty ;
  rdfs:label "Place" ;
  rdfs:comment "Suggested value - bf:Place or madsrdf:Geographic" ;
  dcterms:modified
    "2016-04-21 (New)" ,
    "2021-06-09 (Broadened range [GH19])" ,
    "2025-01-23 (Ontological correction - partially addresses [GH121])"
    ;
  skos:definition "Geographic location or place entity associated with a resource or element of description, such as the place associated with the publication, printing, distribution, issue, release or production of a resource, place of an event." ;
  .

bf:polarity
  a owl:ObjectProperty ;
  rdfs:label "Polarity" ;
  dcterms:modified "2016-04-21 (New)" ;
  rdfs:domain bf:Instance ;
  rdfs:range bf:Polarity ;
  skos:definition "Relationship of the colors and tones in an image to the colors and tones of the object reproduced." ;
  .

bf:precededBy
  a owl:ObjectProperty ;
  rdfs:subPropertyOf bf:relatedTo ;
  rdfs:label "Preceded by" ;
  rdfs:comment
    "Suggested use - With Work or Instance" ,
    "Suggested value - Work or Instance"
    ;
  dcterms:modified
    "2016-04-21 (New)" ,
    "2016-04-29 (added inverse)"
    ;
  owl:inverseOf bf:succeededBy ;
  skos:definition "Resource that precedes the resource being described, e.g., is earlier in time or before in narrative" ;
  .

bf:preferredCitation
  a owl:DatatypeProperty ;
  rdfs:label "Preferred citation" ;
  rdfs:comment "Suggested use - With Work or Instance" ;
  dcterms:modified "2016-04-21 (New)" ;
  rdfs:range rdfs:Literal ;
  skos:definition "Citation to the resource preferred by its custodian of the resource." ;
  .

bf:productionMethod
  a owl:ObjectProperty ;
  rdfs:label "Production method" ;
  dcterms:modified "2016-04-21 (New)" ;
  rdfs:domain bf:Instance ;
  rdfs:range bf:ProductionMethod ;
  skos:definition "Process used to produce a resource." ;
  .

bf:productionStatement
  a owl:DatatypeProperty ;
  rdfs:label "Production statement" ;
  dcterms:modified "2024-07-10 (New [GH124])" ;
  rdfs:domain bf:Instance ;
  rdfs:range rdfs:Literal ;
  skos:definition "Statement related to the production of the resources; usually transcribed." ;
  .

bf:projection
  a owl:ObjectProperty ;
  rdfs:label "Cartographic projection" ;
  dcterms:modified
    "2016-04-21 (New)" ,
    "2017-02-03 (changed from data to object property)"
    ;
  rdfs:domain bf:Cartographic ;
  rdfs:range bf:Projection ;
  skos:definition "Method or system used to represent the surface of the earth or of a celestial sphere on a plane." ;
  .

bf:projectionCharacteristic
  a owl:ObjectProperty ;
  rdfs:label "Projection characteristic" ;
  dcterms:modified
    "2016-04-21 (New)" ,
    "2017-02-03 (fixed typo in property name)"
    ;
  rdfs:domain bf:Instance ;
  rdfs:range bf:ProjectionCharacteristic ;
  skos:definition "Technical specification relating to the projection of a motion picture film." ;
  .

bf:provisionActivity
  a owl:ObjectProperty ;
  rdfs:label "Provision activity" ;
  dcterms:modified
    "2016-04-21 (New)" ,
    "2017-02-03 (revised label and slightly revised definition)"
    ;
  rdfs:domain bf:Instance ;
  rdfs:range bf:ProvisionActivity ;
  skos:definition "Place, name, and/or date information relating to the publication, printing, distribution, issue, release, production, etc. of a resource." ;
  .

bf:provisionActivityStatement
  a owl:DatatypeProperty ;
  rdfs:label "Provider statement" ;
  dcterms:modified "2016-04-21 (New)" ;
  rdfs:domain bf:Instance ;
  rdfs:range rdfs:Literal ;
  skos:definition "Statement relating to providers of a resource; usually transcribed." ;
  .

bf:pubFrequency
  a owl:ObjectProperty ;
  rdfs:label "Publication frequency" ;
  rdfs:comment "Suggested use - With Work or Instance" ;
  dcterms:modified "2021-06-09 (New [GH76])" ;
  rdfs:range bf:PubFrequency ;
  skos:definition "Relates a resource to a publication frequency resource to capture such details as first issue, last issue, status, etc." ;
  .

bf:publicationStatement
  a owl:DatatypeProperty ;
  rdfs:label "Publication statement" ;
  dcterms:modified "2024-07-10 (New [GH124])" ;
  rdfs:domain bf:Instance ;
  rdfs:range rdfs:Literal ;
  skos:definition "Statement related to the publication of the resources; usually transcribed." ;
  .

bf:qualifier
  a owl:DatatypeProperty ;
  rdfs:label "Qualifier" ;
  dcterms:modified
    "2016-04-21 (New)" ,
    "2025-01-23 (Ontological correction - partially addresses [GH121])"
    ;
  rdfs:range rdfs:Literal ;
  skos:definition "Qualifier of information, such as an addition to a title to make it unique or qualifying information associated with an identifier." ;
  .

bf:reductionRatio
  a owl:ObjectProperty ;
  rdfs:label "Reduction ratio" ;
  dcterms:modified "2016-04-21 (New)" ;
  rdfs:domain bf:Instance ;
  rdfs:range bf:ReductionRatio ;
  skos:definition "Size of a micro-image in relation to the original from which it was produced." ;
  .

bf:referencedBy
  a owl:ObjectProperty ;
  rdfs:subPropertyOf bf:relatedTo ;
  rdfs:label "Referenced by" ;
  rdfs:comment
    "Suggested use - With Work, Instance or Item" ,
    "Suggested value - Work, Instance or Item"
    ;
  dcterms:modified
    "2016-04-21 (New)" ,
    "2016-04-29 (added inverse)"
    ;
  owl:inverseOf bf:references ;
  skos:definition "Resource that references the described resource" ;
  .

bf:references
  a owl:ObjectProperty ;
  rdfs:subPropertyOf bf:relatedTo ;
  rdfs:label "References" ;
  rdfs:comment
    "Suggested use - With Work, Instance or Item" ,
    "Suggested value - Work, Instance or Item"
    ;
  dcterms:modified
    "2016-04-21 (New)" ,
    "2016-04-29 (added inverse)"
    ;
  owl:inverseOf bf:referencedBy ;
  skos:definition "Resource that is referenced by the described resource" ;
  .

bf:relatedTo
  a owl:SymmetricProperty ;
  rdfs:label "Related resource" ;
  dcterms:modified
    "2016-04-21 (New)" ,
    "2021-06-09 (Modified definition [GH2])" ,
    "2025-01-23 (Ontological correction - partially addresses [GH121])"
    ;
  skos:definition "Any relationship between Work, Instance, Item, and Event resources" ;
  .

bf:relation
  a owl:ObjectProperty ;
  rdfs:label "Relation" ;
  rdfs:comment "Suggested use - With Work, Instance or Item" ;
  dcterms:modified "2022-07-10 (New [GH116])" ;
  rdfs:range bf:Relation ;
  skos:definition "Associated resource and its relationship to the resource being described" ;
  .

bf:relationship
  a owl:ObjectProperty ;
  rdfs:label "Relationship" ;
  dcterms:modified "2022-07-10 (New [GH116])" ;
  rdfs:domain bf:Relation ;
  rdfs:range bf:Relationship ;
  skos:definition "Type of relationship between resources" ;
  .

bf:relief
  a owl:ObjectProperty ;
  rdfs:label "Relief" ;
  dcterms:modified "2023-11-30 (New [GH104])" ;
  rdfs:domain bf:Instance ;
  rdfs:range bf:Relief ;
  skos:definition "Relief term specified on a cartographic resource" ;
  .

bf:replacedBy
  a owl:ObjectProperty ;
  rdfs:subPropertyOf bf:succeededBy ;
  rdfs:label "Replaced by" ;
  rdfs:comment
    "Suggested use - With Work or Instance" ,
    "Suggested value - Work or Instance"
    ;
  dcterms:modified
    "2016-04-21 (New)" ,
    "2016-04-29 (added inverse, updated range)" ,
    "2022-10-03 (corrected label [GH85])"
    ;
  owl:inverseOf bf:replacementOf ;
  skos:definition "Later resource used in place of an earlier resource, usually because the later resource contains updated or new information" ;
  .

bf:replacementOf
  a owl:ObjectProperty ;
  rdfs:subPropertyOf bf:precededBy ;
  rdfs:label "Replacement of" ;
  rdfs:comment
    "Suggested use - With Work or Instance" ,
    "Suggested value - Work or Instance"
    ;
  dcterms:modified
    "2016-04-21 (New)" ,
    "2016-04-29 (added inverse, updated range)" ,
    "2022-10-03 (corrected label [GH85])"
    ;
  owl:inverseOf bf:replacedBy ;
  skos:definition "Earlier resource whose content has been replaced by a later resource, usually because the later resource contains updated or new information" ;
  .

bf:reproductionOf
  a owl:ObjectProperty ;
  rdfs:subPropertyOf bf:hasEquivalent ;
  rdfs:label "Reproduction of" ;
  dcterms:modified
    "2016-04-21 (New)" ,
    "2016-04-29 (added inverse)"
    ;
  rdfs:domain bf:Instance ;
  rdfs:range bf:Instance ;
  owl:inverseOf bf:hasReproduction ;
  skos:definition "Resource that is a reproduction of another Resource" ;
  .

bf:responsibilityStatement
  a owl:DatatypeProperty ;
  rdfs:label "Creative responsibility statement" ;
  dcterms:modified "2016-04-21 (New)" ;
  rdfs:domain bf:Instance ;
  rdfs:range rdfs:Literal ;
  skos:definition "Statement relating to any persons, families, or corporate bodies responsible for the creation of, or contributing to the content of a resource; usually transcribed." ;
  .

bf:review
  a owl:ObjectProperty ;
  rdfs:label "Review content" ;
  rdfs:comment "Suggested use - With Work or Instance" ;
  dcterms:modified "2016-04-21 (New)" ;
  rdfs:range bf:Review ;
  skos:definition "Review of a resource." ;
  .

bf:role
  a owl:ObjectProperty ;
  rdfs:label "Contributor role" ;
  dcterms:modified
    "2016-04-21 (New)" ,
    "2017-02-03 (Changed from data to object property, adjusted label and definition)"
    ;
  rdfs:domain bf:Contribution ;
  rdfs:range bf:Role ;
  skos:definition "Function provided by a contributor, e.g., author, illustrator, etc." ;
  .

bf:scale
  a owl:ObjectProperty ;
  rdfs:label "Scale" ;
  rdfs:comment "Suggested use - With Work or Instance" ;
  dcterms:modified
    "2016-04-21 (New)" ,
    "2017-02-03 (changed from data to object property)"
    ;
  rdfs:range bf:Scale ;
  skos:definition "Ratio of the dimensions of a form contained or embodied in a resource to the dimensions of the entity it represents, e.g., for images or cartographic resources." ;
  .

bf:schedulePart
  a owl:DatatypeProperty ;
  rdfs:label "Classification designation" ;
  dcterms:modified "2016-04-21 (New)" ;
  rdfs:domain bf:Classification ;
  rdfs:range rdfs:Literal ;
  skos:definition "Designates whether the classification number is from the standard or optional part of a schedule or table." ;
  .

bf:separatedFrom
  a owl:ObjectProperty ;
  rdfs:subPropertyOf bf:precededBy ;
  rdfs:label "Separated from" ;
  rdfs:comment
    "Suggested use - With Work or Instance" ,
    "Suggested value - Work or Instance"
    ;
  dcterms:modified
    "2016-04-21 (New)" ,
    "2016-04-29 (added inverse, updated range)"
    ;
  owl:inverseOf bf:continuedInPartBy ;
  skos:definition "Resource that spun off a part of its content to form a new resource" ;
  .

bf:seriesEnumeration
  a owl:DatatypeProperty ;
  rdfs:label "Series enumeration" ;
  rdfs:comment "Suggested use - With Work or Instance" ;
  dcterms:modified
    "2016-04-21 (New)" ,
    "2024-07-10 (changed domain [GH100])"
    ;
  rdfs:range rdfs:Literal ;
  skos:definition "Series enumeration of the resource; usually transcribed." ;
  .

bf:seriesOf
  a owl:ObjectProperty ;
  rdfs:subPropertyOf bf:hasPart ;
  rdfs:label "Series container of" ;
  rdfs:comment
    "Suggested use - With Work or Instance" ,
    "Suggested value - Work or Instance"
    ;
  dcterms:modified
    "2016-04-21 (New)" ,
    "2016-04-29 (added inverse, updated range)" ,
    "2024-07-10 (updated definition [GF106])"
    ;
  owl:inverseOf bf:hasSeries ;
  skos:definition "Relation between a larger resource and the resources it encompasses, forming a series, the title of the larger resource appears on the parts" ;
  .

bf:seriesStatement
  a owl:DatatypeProperty ;
  rdfs:label "Series statement" ;
  dcterms:modified "2016-04-21 (New)" ;
  rdfs:domain bf:Instance ;
  rdfs:range rdfs:Literal ;
  skos:definition "Statement of the series the resource is in; usually transcribed; includes the ISSN if applicable." ;
  .

bf:shelfMark
  a owl:ObjectProperty ;
  rdfs:label "Shelf mark" ;
  dcterms:modified "2016-04-21 (New)" ;
  rdfs:domain bf:Item ;
  rdfs:range bf:ShelfMark ;
  skos:definition "Piece identifier, such as a call or other type of number." ;
  .

bf:soundCharacteristic
  a owl:ObjectProperty ;
  rdfs:label "Sound characteristic" ;
  dcterms:modified
    "2016-04-21 (New)" ,
    "2016-04-21 (fixed name and range typos)"
    ;
  rdfs:domain bf:Instance ;
  rdfs:range bf:SoundCharacteristic ;
  skos:definition "Technical specification relating to the encoding of sound in a resource." ;
  .

bf:soundContent
  a owl:ObjectProperty ;
  rdfs:label "Sound content" ;
  rdfs:comment "Suggested use - With Work or Instance" ;
  dcterms:modified "2016-04-21 (New)" ;
  rdfs:range bf:SoundContent ;
  skos:definition "Indication of whether the production of sound is an integral part of the resource." ;
  .

bf:source
  a owl:ObjectProperty ;
  rdfs:label "Source" ;
  rdfs:comment "Suggested value - bf:Organization or bf:Assigner" ;
  dcterms:modified
    "2016-04-21 (New)" ,
    "2021-06-09 (Broadened range [GH63])" ,
    "2025-01-23 (Ontological correction - partially addresses [GH121])"
    ;
  skos:definition "Resource from which value or label came or was derived, such as the formal source/scheme from which a classification number is taken or derived, list from which an agent name is taken or derived, source within which an identifier is unique." ;
  .

bf:spanEnd
  a owl:DatatypeProperty ;
  rdfs:label "Classification number span end" ;
  dcterms:modified "2016-04-21 (New)" ;
  rdfs:domain bf:Classification ;
  rdfs:range rdfs:Literal ;
  skos:definition "Ending number of classification number span." ;
  .

bf:splitInto
  a owl:ObjectProperty ;
  rdfs:subPropertyOf bf:succeededBy ;
  rdfs:label "Split into" ;
  rdfs:comment
    "Suggested use - With Work or Instance" ,
    "Suggested value - Work or Instance"
    ;
  dcterms:modified
    "2016-04-21 (New)" ,
    "2016-04-29 (added inverse, updated range)"
    ;
  owl:inverseOf bf:continuesInPart ;
  skos:definition "One of two or more resources resulting from the division of an earlier resource into separate resources" ;
  .

bf:status
  a owl:ObjectProperty ;
  rdfs:label "Status" ;
  dcterms:modified
    "2016-04-21 (New)" ,
    "2025-01-23 (Ontological correction - partially addresses [GH121])"
    ;
  rdfs:range bf:Status ;
  skos:definition "Designation of the validity or position of something, such as indication that the classification number is canceled or invalid, circulation availability of an item, indication of whether the identifier is canceled or invalid." ;
  .

bf:subject
  a owl:ObjectProperty ;
  rdfs:label "Subject" ;
  rdfs:comment
    "Suggested use - With Work, Instance, Item or Event" ,
    "Suggested value - bf:Agent or bf:Topic or bf:Hub"
    ;
  dcterms:modified
    "2016-04-21 (New)" ,
    "2021-06-09 (Broadened domain [GH21])" ,
    "2025-01-23 (Ontological correction - partially addresses [GH121])"
    ;
  skos:definition "Subject term(s) describing a resource." ;
  .

bf:subjectOf
  a owl:ObjectProperty ;
  rdfs:label "Subject of" ;
  rdfs:comment
    "Suggested use - With bf:Agent or bf:Topic or bf:Hub" ,
    "Suggested value - Work, Instance, Item or Event"
    ;
  dcterms:modified
    "2021-06-09 (New [GH20])" ,
    "2025-01-23 (Ontological correction - partially addresses [GH121])"
    ;
  skos:definition "Relates a subject to that which it describes." ;
  .

bf:sublocation
  a owl:ObjectProperty ;
  rdfs:label "Held in sublocation" ;
  dcterms:modified "2016-04-21 (New)" ;
  rdfs:domain bf:Item ;
  rdfs:range bf:Sublocation ;
  skos:definition "Specific place within the holding entity where the item is located or made available." ;
  .

bf:subseriesEnumeration
  a owl:DatatypeProperty ;
  rdfs:label "Subseries enumeration" ;
  dcterms:modified "2016-04-21 (New)" ;
  rdfs:domain bf:Instance ;
  rdfs:range rdfs:Literal ;
  skos:definition "Subseries enumeration of the resource; usually transcribed." ;
  .

bf:subseriesOf
  a owl:ObjectProperty ;
  rdfs:subPropertyOf bf:hasPart ;
  rdfs:label "Subseries of" ;
  rdfs:comment
    "Suggested use - With Work or Instance" ,
    "Suggested value - Work or Instance"
    ;
  dcterms:modified
    "2016-04-21 (New)" ,
    "2016-04-29 (added inverse, updated range)" ,
    "2024-07-10 (updated definition [GF106])"
    ;
  owl:inverseOf bf:hasSubseries ;
  skos:definition "Relation between a Series resource and the resources it encompasses, forming a Subseries; the Series resource itself has a relation with a larger resource, of which it is a part" ;
  .

bf:subseriesStatement
  a owl:DatatypeProperty ;
  rdfs:label "Subseries statement" ;
  dcterms:modified "2016-04-21 (New)" ;
  rdfs:domain bf:Instance ;
  rdfs:range rdfs:Literal ;
  skos:definition "Statement of the subseries the resource is in; usually transcribed; includes the ISSN if applicable." ;
  .

bf:subtitle
  a owl:DatatypeProperty ;
  rdfs:label "Subtitle" ;
  dcterms:modified "2016-04-21 (New)" ;
  rdfs:domain bf:Title ;
  rdfs:range rdfs:Literal ;
  skos:definition "Word, character, or group of words and/or characters that contains the remainder of the title after the main title. Possible title component." ;
  .

bf:succeededBy
  a owl:ObjectProperty ;
  rdfs:subPropertyOf bf:relatedTo ;
  rdfs:label "Succeeded by" ;
  rdfs:comment
    "Suggested use - With Work or Instance" ,
    "Suggested value - Work or Instance"
    ;
  dcterms:modified
    "2016-04-21 (New)" ,
    "2016-04-29 (added inverse)"
    ;
  owl:inverseOf bf:precededBy ;
  skos:definition "Resource that succeeds the resource being described, e.g., later in time or after in a narrative" ;
  .

bf:summary
  a owl:ObjectProperty ;
  rdfs:label "Summary content" ;
  rdfs:comment "Suggested use - With Work or Instance" ;
  dcterms:modified "2016-04-21 (New)" ;
  rdfs:range bf:Summary ;
  skos:definition "Summary or abstract of the resource described." ;
  .

bf:supplement
  a owl:ObjectProperty ;
  rdfs:subPropertyOf bf:accompaniedBy ;
  rdfs:label "Supplement" ;
  rdfs:comment
    "Suggested use - With Work or Instance" ,
    "Suggested value - Work or Instance"
    ;
  dcterms:modified
    "2016-04-21 (New)" ,
    "2016-04-29 (added inverse, updated range)"
    ;
  owl:inverseOf bf:supplementTo ;
  skos:definition "Resource that updates or otherwise complements the predominant resource" ;
  .

bf:supplementTo
  a owl:ObjectProperty ;
  rdfs:subPropertyOf bf:accompanies ;
  rdfs:label "Supplement to" ;
  rdfs:comment
    "Suggested use - With Work or Instance" ,
    "Suggested value - Work or Instance"
    ;
  dcterms:modified
    "2016-04-21 (New)" ,
    "2016-04-29 (added inverse, updated range)"
    ;
  owl:inverseOf bf:supplement ;
  skos:definition "Resource that is updated or otherwise complemented by the augmenting resource" ;
  .

bf:supplementaryContent
  a owl:ObjectProperty ;
  rdfs:label "Supplementary material" ;
  rdfs:comment "Suggested use - With Work or Instance" ;
  dcterms:modified "2016-04-21 (New)" ;
  rdfs:range bf:SupplementaryContent ;
  skos:definition "Material such as an index, bibliography, appendix intended to supplement the primary content of a resource." ;
  .

bf:systemRequirement
  a owl:ObjectProperty ;
  rdfs:label "Equipment or system requirements" ;
  dcterms:modified
    "2016-04-21 (New)" ,
    "2017-02-06 (Changed from data to object property, changed property name from plural to singular)"
    ;
  rdfs:domain bf:Instance ;
  rdfs:range bf:SystemRequirement ;
  skos:definition "Equipment or system requirement beyond what is normal and obvious for the type of carrier or type of file, such as make and model of equipment or hardware, operating system, amount of memory, programming language, other necessary software, any plug-ins or peripherals required to play, view, or run the resource, etc." ;
  .

bf:table
  a owl:DatatypeProperty ;
  rdfs:label "Classification table identification" ;
  dcterms:modified "2016-04-21 (New)" ;
  rdfs:domain bf:Classification ;
  rdfs:range rdfs:Literal ;
  skos:definition "Number of the table from which the classification number in a subdivision entry is taken, e.g., a DDC table." ;
  .

bf:tableOfContents
  a owl:ObjectProperty ;
  rdfs:label "Table of contents content" ;
  rdfs:comment "Suggested use - With Work or Instance" ;
  dcterms:modified "2016-04-21 (New)" ;
  rdfs:range bf:TableOfContents ;
  skos:definition "Table of contents of the described resource." ;
  .

bf:tableSeq
  a owl:DatatypeProperty ;
  rdfs:label "Classification table sequence number" ;
  dcterms:modified "2016-04-21 (New)" ;
  rdfs:domain bf:Classification ;
  rdfs:range rdfs:Literal ;
  skos:definition "Sequence number or other identifier for an internal classification sub arrangement or add in a classification scheme." ;
  .

bf:temporalCoverage
  a owl:DatatypeProperty ;
  rdfs:label "Temporal coverage" ;
  dcterms:modified "2016-04-21 (New)" ;
  rdfs:domain bf:Work ;
  rdfs:range rdfs:Literal ;
  skos:definition "Time period coverage of the content of the resource." ;
  .

bf:title
  a owl:ObjectProperty ;
  rdfs:label "Title resource" ;
  rdfs:comment "Suggested use - With Work, Instance, Item or Event" ;
  dcterms:modified
    "2016-04-21 (New)" ,
    "2021-06-09 (Broadened domain [GH23])"
    ;
  rdfs:range bf:Title ;
  skos:definition "Name given to a resource." ;
  .

bf:titleOf
  a owl:ObjectProperty ;
  rdfs:label "Title of" ;
  rdfs:comment "Suggested value - Work, Instance, Item or Event" ;
  dcterms:modified "2021-06-09 (New [GH22])" ;
  rdfs:domain bf:Title ;
  skos:definition "Relates a title resource to that which it is the title of." ;
  .

bf:translation
  a owl:ObjectProperty ;
  rdfs:subPropertyOf bf:hasDerivative ;
  rdfs:label "Translation as" ;
  rdfs:comment
    "Suggested use - With Work or Instance" ,
    "Suggested value - Work or Instance"
    ;
  dcterms:modified
    "2016-04-21 (New)" ,
    "2016-04-29 (added inverse, updated range)" ,
    "2017-02-03 (corrected subproperty)"
    ;
  owl:inverseOf bf:translationOf ;
  skos:definition "Resource that translates the text of the source entity into a language different from that of the original" ;
  .

bf:translationOf
  a owl:ObjectProperty ;
  rdfs:subPropertyOf bf:derivativeOf ;
  rdfs:label "Translation of" ;
  rdfs:comment
    "Suggested use - With Work or Instance" ,
    "Suggested value - Work or Instance"
    ;
  dcterms:modified
    "2016-04-21 (New)" ,
    "2016-04-29 (added inverse, updated range)" ,
    "2017-02-03 (corrected subproperty)"
    ;
  owl:inverseOf bf:translation ;
  skos:definition "Resource that has been translated, i.e., the text is expressed in a language different from that of the original resource" ;
  .

bf:unit
  a owl:ObjectProperty ;
  rdfs:label "Type of unit" ;
  dcterms:modified
    "2016-04-21 (New)" ,
    "2025-01-23 (Ontological correction - partially addresses [GH121])"
    ;
  rdfs:range bf:Unit ;
  skos:definition "Units in which a value is expressed, such as the physical or logical constituent of a resource (e.g., a volume, audiocassette, film reel, a map, a digital file)." ;
  .

bf:usageAndAccessPolicy
  a owl:ObjectProperty ;
  rdfs:label "Use and access condition" ;
  rdfs:comment "Suggested use - With Work, Instance or Item" ;
  dcterms:modified "2016-04-21 (New)" ;
  rdfs:range bf:UsageAndAccessPolicy ;
  skos:definition "General statement of allowances and restrictions on access to a resource, including retention, reproduction, access, and lending." ;
  .

bf:validDate
  a owl:DatatypeProperty ;
  rdfs:subPropertyOf bf:date ;
  rdfs:label "Valid date" ;
  dcterms:modified "2022-10-03 (New [GH68])" ;
  rdfs:domain bf:Work ;
  rdfs:range rdfs:Literal ;
  skos:definition "The date or date range during which the resource is accurate." ;
  .

bf:variantType
  a owl:DatatypeProperty ;
  rdfs:label "Variant title type" ;
  dcterms:modified "2016-04-21 (New)" ;
  rdfs:domain bf:VariantTitle ;
  rdfs:range rdfs:Literal ;
  skos:definition "Type of title variation, e.g., acronym, cover, spine, earlier, later, series version." ;
  .

bf:version
  a owl:DatatypeProperty ;
  rdfs:label "Version" ;
  dcterms:modified "2016-04-21 (New)" ;
  rdfs:domain bf:Work ;
  rdfs:range rdfs:Literal ;
  skos:definition "Term or terms that identify works such as arranged for music, vulgate for religious work, etc." ;
  .

bf:videoCharacteristic
  a owl:ObjectProperty ;
  rdfs:label "Video characteristic" ;
  dcterms:modified "2016-04-21 (New)" ;
  rdfs:domain bf:Instance ;
  rdfs:range bf:VideoCharacteristic ;
  skos:definition "Technical specification relating to the encoding of video images in a resource" ;
  .

bf:voice
  a owl:ObjectProperty ;
  rdfs:label "Voice" ;
  dcterms:modified "2016-04-21 (New)" ;
  rdfs:domain bf:Work ;
  rdfs:range bf:MusicVoice ;
  skos:definition "Voice for which a musical work is appropriate, such as soprano, tenor, mixed." ;
  .

bf:voiceType
  a owl:DatatypeProperty ;
  rdfs:label "Type of voice" ;
  dcterms:modified "2016-04-21 (New)" ;
  rdfs:domain bf:MusicVoice ;
  rdfs:range rdfs:Literal ;
  skos:definition "Specific type of voice group, such as chorus, solo." ;
  .

